Escallon/LR_Parsing/Generalized_Pushdown_Automata.thy
@@ -1,22 +1,23 @@
-theory N_Pushdown_Automata
+theory Generalized_Pushdown_Automata
   imports
     Auxiliary
     Pushdown_Automata.Pushdown_Automata 
 begin
 
-record ('q, 'a) npda = states :: "'q set"
+record ('q, 'a) gpda = states :: "'q set"
                        init   :: 'q
                        final  :: "'q set"
                        nxt    :: "('q list \<times> 'a \<times> 'q list) set"
                        eps    :: "('q list \<times> 'q list) set"
+                      
 
 type_synonym ('q, 'a) config = "'q list \<times> 'a list"
 
 (* Placeholder, should be states M 
 consts Q :: "'s::fresh0 set" *)
 
-locale npda =
-  fixes M :: "('q, 'a) npda"
+locale gpda =
+  fixes M :: "('q, 'a) gpda"
   assumes init:       "init M \<in> states M"
       and final:      "final M \<subseteq> states M"
       and nxt:        "(ps, a, qs) \<in> nxt M \<Longrightarrow> ps \<noteq> [] \<and> qs \<noteq> [] 
@@ -53,12 +54,36 @@ abbreviation steps :: "('q,'a) config \<Rightarrow> ('q,'a) config \<Rightarrow>
 abbreviation stepn :: "('q,'a) config \<Rightarrow> nat \<Rightarrow> ('q,'a) config \<Rightarrow> bool" (\<open>_ \<turnstile>'(_') _\<close> 55) where
   "c\<^sub>0 \<turnstile>(n) c\<^sub>1 \<equiv> (step ^^ n) c\<^sub>0 c\<^sub>1"
 
+lemma reachable_imp_substring:
+  assumes "(ps, w) \<turnstile>* (qs, v)"
+  obtains u where "w = u @ v"
+  using assms proof (induction "(qs, v)" arbitrary: qs v thesis rule: rtranclp_induct)
+  case (step y)
+  from step(2) show ?case proof cases
+    case (step_nxt rs a ss ts)
+    with step(3)[of _ "a # v"] step(4)[of "_ @ [a]"] show ?thesis by auto
+  qed (use step in auto)
+qed simp
+
+lemma steps_states_imp_states:
+  assumes "(ps, u) \<turnstile>* (qs, v)"
+    "set ps \<subseteq> states M"
+  shows "set qs \<subseteq> states M"
+  using assms by (induction rule: rtranclp_induct2)
+    (use step_states_imp_states in blast)+
+
+corollary steps_init_imp_states:
+  assumes "([init M], u) \<turnstile>* (qs, v)"
+  shows "set qs \<subseteq> states M"
+  using steps_states_imp_states[OF assms] init by auto
+
+
 definition Lang :: "'a list set" where
   "Lang \<equiv> {w. \<exists>f \<in> final M. ([init M], w) \<turnstile>* ([f], [])}"
 
 (*
 
-Towards npda \<Longrightarrow> pda
+Towards gpda \<Longrightarrow> pda
 
 definition states_of_eps :: "('s list \<times> 's list) set \<Rightarrow> 's set" where
   "states_of_eps \<E> \<equiv> \<Union>(ps, qs) \<in> \<E>. set ps \<union> set qs"
@@ -88,8 +113,8 @@ section \<open>Equivalence with PDAs\<close>
 
 datatype ('a, 'b, 'c) sum3 = Qtyp 'a | Styp 'b | Q'typ 'c
 
-definition npda_of_pda :: "('q, 'a, 's) pda \<Rightarrow> (('q, 's, 'r::fresh0) sum3, 'a) npda" where
-  "npda_of_pda M \<equiv> let 
+definition gpda_of_pda :: "('q, 'a, 's) pda \<Rightarrow> (('q, 's, 'r::fresh0) sum3, 'a) gpda" where
+  "gpda_of_pda M \<equiv> let 
     Q\<^sub>M = UNIV :: 'q set;
     \<Gamma> = UNIV :: 's set; 
     q\<^sub>0 = fresh0 ({}::'r set);
@@ -100,31 +125,31 @@ definition npda_of_pda :: "('q, 'a, 's) pda \<Rightarrow> (('q, 's, 'r::fresh0) 
         \<union> {([Qtyp f], [Q'typ q\<^sub>f])|f. f \<in> final_states M}
   in \<lparr>states = Qtyp ` Q\<^sub>M \<union> Styp ` \<Gamma> \<union> Q'typ ` {q\<^sub>0, q\<^sub>f}, init = Q'typ q\<^sub>0, final = {Q'typ q\<^sub>f}, nxt = \<Delta>, eps = \<E>\<rparr> "
 
-lemma states_npda_of_pda [simp]:
-  "states ((npda_of_pda M)::(('q, 's, 'r::fresh0) sum3, 'a) npda) 
+lemma states_gpda_of_pda [simp]:
+  "states ((gpda_of_pda M)::(('q, 's, 'r::fresh0) sum3, 'a) gpda) 
     = (let  q\<^sub>0 = fresh0 ({}::'r set);
       q\<^sub>f = fresh0 {q\<^sub>0} in 
     (Qtyp ` (UNIV :: 'q set)) \<union> (Styp ` (UNIV :: 's set)) \<union> (Q'typ ` {q\<^sub>0, q\<^sub>f}))"
-  unfolding npda_of_pda_def by (meson npda.select_convs(1))
+  unfolding gpda_of_pda_def by (meson gpda.select_convs(1))
 
-lemma npda_of_pda_states_contain_pda_states_stack:
-  "Qtyp ` UNIV \<union> Styp ` UNIV \<subseteq> states (npda_of_pda M)"
-  using states_npda_of_pda by (metis sup_ge1)
+lemma gpda_of_pda_states_contain_pda_states_stack:
+  "Qtyp ` UNIV \<union> Styp ` UNIV \<subseteq> states (gpda_of_pda M)"
+  using states_gpda_of_pda by (metis sup_ge1)
 
-lemma init_npda_of_pda [simp]:
-  "init ((npda_of_pda M)::(('q, 's, 'r::fresh0) sum3, 'a) npda) 
+lemma init_gpda_of_pda [simp]:
+  "init ((gpda_of_pda M)::(('q, 's, 'r::fresh0) sum3, 'a) gpda) 
     = Q'typ (fresh0 ({}::'r set))"
-  unfolding npda_of_pda_def by (meson npda.select_convs(2))
+  unfolding gpda_of_pda_def by (meson gpda.select_convs(2))
 
-lemma final_npda_of_pda[simp]:
-  "final ((npda_of_pda M)::(('q, 's, 'r::fresh0) sum3, 'a) npda)
+lemma final_gpda_of_pda[simp]:
+  "final ((gpda_of_pda M)::(('q, 's, 'r::fresh0) sum3, 'a) gpda)
     = {Q'typ (fresh0 {fresh0 ({}::'r set)})}"
-  unfolding npda_of_pda_def by (meson npda.select_convs(3))
+  unfolding gpda_of_pda_def by (meson gpda.select_convs(3))
 
-lemma nxt_npda_of_pda[simp]:
-  "nxt (npda_of_pda M) = 
+lemma nxt_gpda_of_pda[simp]:
+  "nxt (gpda_of_pda M) = 
     {([Qtyp p, Styp Z], a, Qtyp q # map Styp \<gamma>)|p Z a q \<gamma>. (q, \<gamma>) \<in> delta M p a Z}"
-  unfolding npda_of_pda_def by (meson npda.select_convs(4))
+  unfolding gpda_of_pda_def by (meson gpda.select_convs(4))
 
 definition delta_rel :: "('q, 'a, 's) pda \<Rightarrow> ('q \<times> 's \<times> 'a \<times> 'q \<times> 's list) set" where
   "delta_rel M \<equiv> {(p, Z, a, q, \<gamma>)|p Z a q \<gamma>. (q, \<gamma>) \<in> delta M p a Z}"
@@ -142,72 +167,72 @@ proof -
     by (meson finite_SigmaI finite_UNIV finite_subset)
 qed
 
-lemma bij_betw_delta_rel_npda_of_pda_nxt:
+lemma bij_betw_delta_rel_gpda_of_pda_nxt:
   "bij_betw (\<lambda>(p, Z, a, q, \<gamma>). ([Qtyp p, Styp Z], a, Qtyp q # map Styp \<gamma>)) 
-    (delta_rel M) (nxt (npda_of_pda M))"
+    (delta_rel M) (nxt (gpda_of_pda M))"
   (is "bij_betw ?f _ _")
 proof -
   have "inj_on ?f (delta_rel M)"
     by standard (auto, metis list.inj_map_strong sum3.inject(2))
-  moreover have "?f ` (delta_rel M) = (nxt (npda_of_pda M))"
-    unfolding delta_rel_def nxt_npda_of_pda by (standard; standard) force+
+  moreover have "?f ` (delta_rel M) = (nxt (gpda_of_pda M))"
+    unfolding delta_rel_def nxt_gpda_of_pda by (standard; standard) force+
   ultimately show ?thesis unfolding bij_betw_def by presburger
 qed
 
 
-lemma eps_npda_of_pda[simp]:
-  "eps ((npda_of_pda M)::(('q, 's, 'r::fresh0) sum3, 'a) npda) = 
+lemma eps_gpda_of_pda[simp]:
+  "eps ((gpda_of_pda M)::(('q, 's, 'r::fresh0) sum3, 'a) gpda) = 
   (let  q\<^sub>0 = fresh0 ({}::'r set);
         q\<^sub>f = fresh0 {q\<^sub>0} in 
     {([Qtyp p, Styp Z], Qtyp q # map Styp \<gamma>)|p Z q \<gamma>. 
         (q, \<gamma>) \<in> delta_eps M p Z} \<union> {([Q'typ q\<^sub>0], [Qtyp (init_state M), Styp (init_symbol M)])}
         \<union> {([Qtyp f], [Q'typ q\<^sub>f])|f. f \<in> final_states M})"
-  unfolding npda_of_pda_def by (meson npda.select_convs(5))
+  unfolding gpda_of_pda_def by (meson gpda.select_convs(5))
 
 
-lemma npda_of_pda_nxt_imp_two:
-  assumes "(ps, a, qs) \<in> nxt (npda_of_pda M)"
+lemma gpda_of_pda_nxt_imp_two:
+  assumes "(ps, a, qs) \<in> nxt (gpda_of_pda M)"
   shows "\<exists>p Z. ps = [Qtyp p, Styp Z]"
-  using assms unfolding nxt_npda_of_pda by blast
+  using assms unfolding nxt_gpda_of_pda by blast
 
 
-lemma npda_of_pda_nxt_imp_pda_delta:
-  assumes "(ps, a, qs) \<in> nxt (npda_of_pda M)"
+lemma gpda_of_pda_nxt_imp_pda_delta:
+  assumes "(ps, a, qs) \<in> nxt (gpda_of_pda M)"
   obtains p Z q \<gamma> where "ps = [Qtyp p, Styp Z]" "qs = Qtyp q # map Styp \<gamma>" "(q, \<gamma>) \<in> delta M p a Z"
-  using assms unfolding nxt_npda_of_pda by blast
+  using assms unfolding nxt_gpda_of_pda by blast
 
 lemma
   assumes "pda P"
-  shows "npda (npda_of_pda P)"
+  shows "gpda (gpda_of_pda P)"
 proof (unfold_locales, goal_cases)
   case 1
-  then show ?case using init_npda_of_pda states_npda_of_pda
+  then show ?case using init_gpda_of_pda states_gpda_of_pda
     by (metis Un_iff image_eqI insertCI)
 next
   case 2
-  then show ?case using states_npda_of_pda final_npda_of_pda 
+  then show ?case using states_gpda_of_pda final_gpda_of_pda 
     by (smt (verit, ccfv_threshold) Un_iff empty_iff image_eqI insert_iff subsetI)
 next
   case (3 ps a qs)
-  from npda_of_pda_nxt_imp_pda_delta[OF this] obtain p Z q \<gamma> where ps_qs_defs:
+  from gpda_of_pda_nxt_imp_pda_delta[OF this] obtain p Z q \<gamma> where ps_qs_defs:
     "ps = [Qtyp p, Styp Z]"
     "qs = Qtyp q # map Styp \<gamma>"
     by metis
   hence "set qs \<subseteq> Qtyp ` UNIV \<union> Styp ` UNIV" "set ps \<subseteq> Qtyp ` UNIV \<union> Styp ` UNIV"
     by auto
   with ps_qs_defs show ?case 
-    using npda_of_pda_states_contain_pda_states_stack by auto
+    using gpda_of_pda_states_contain_pda_states_stack by auto
 next
   case (4 ps qs)
   then show ?case sorry
 next
   case 5
-  then show ?case unfolding states_npda_of_pda 
+  then show ?case unfolding states_gpda_of_pda 
     by (metis finite.simps finite_UNIV finite_Un finite_imageI)
 next
   case 6
   then show ?case 
-    using pda_imp_finite_delta_rel[OF assms] bij_betw_delta_rel_npda_of_pda_nxt
+    using pda_imp_finite_delta_rel[OF assms] bij_betw_delta_rel_gpda_of_pda_nxt
       bij_betw_finite by auto
 next
   case 7
@@ -215,9 +240,9 @@ next
 qed
 
 
-theorem Cfg_imp_npda:
+theorem Cfg_imp_gpda:
   fixes G :: "('n, 't) Cfg"
-  obtains M :: "('q, 't) npda" where "npda.Lang M = LangS G" 
+  obtains M :: "('q, 't) gpda" where "gpda.Lang M = LangS G" 
   sorry
 
 
