Escallon/LR_Parsing/LR_Parser.thy
@@ -1,6 +1,6 @@
 theory LR_Parser 
   imports
-    N_Pushdown_Automata
+    Generalized_Pushdown_Automata
     Item_Pushdown_Automata
     Rightmost_Chain
     Wlog.Wlog
@@ -96,6 +96,12 @@ lemma eps_char_fa [simp]:
   "nfa.eps char_fa 
     = {([X \<rightarrow> \<alpha> \<cdot> Nt Y # \<beta>], [Y \<rightarrow> [] \<cdot> \<gamma>]) | X \<alpha> Y \<beta> \<gamma>. (X, \<alpha> @ Nt Y # \<beta>) \<in> Prods G' \<and> (Y, \<gamma>) \<in> Prods G'}"
   unfolding char_fa_def by (meson nfa.select_convs(5))
+
+lemma eps_char_faE [elim]:
+  assumes "(i, j) \<in> nfa.eps char_fa"
+  obtains X \<alpha> Y \<beta> \<gamma> where "(X, \<alpha> @ Nt Y # \<beta>) \<in> Prods G'" "(Y, \<gamma>) \<in> Prods G'"
+    "i = [X \<rightarrow> \<alpha> \<cdot> Nt Y # \<beta>]" "j = [Y \<rightarrow> [] \<cdot> \<gamma>]"
+  using assms unfolding eps_char_fa by blast
 
 lemma eps_char_fa_subst_states:
   "nfa.eps char_fa \<subseteq> nfa.states char_fa \<times> nfa.states char_fa"
@@ -304,6 +310,7 @@ next
     by simp
   finally show ?case using step.prems[of "x@w"] by auto
 qed
+
 
 
 end
@@ -602,6 +609,60 @@ proof (induction rule: converse_rtrancl_induct)
   with char_fa.step_eps[OF this(1), of \<zeta>] show ?case by simp
 qed simp
 
+lemma char_step_left_nonempty_imp_not_eps:
+  assumes "([A \<rightarrow> \<alpha> \<cdot> \<beta>], X # \<gamma>) \<turnstile>c ([B \<rightarrow> \<delta> @ [Y] \<cdot> \<zeta>], \<eta>)"
+  obtains \<beta>' where "\<beta> = X # \<beta>'" "([B \<rightarrow> \<delta> @ [Y] \<cdot> \<zeta>], \<eta>) = ([A \<rightarrow> \<alpha> @ [X] \<cdot> \<beta>'], \<gamma>)"
+  using assms by cases fast+
+
+lemma char_eps_impossible:
+  assumes "([A \<rightarrow> \<alpha> \<cdot> \<beta>], []) \<turnstile>c ([B \<rightarrow> \<delta> @ [Y] \<cdot> \<zeta>], \<eta>)"
+  shows False using assms by cases auto
+
+lemma char_reaches_left_empty_imp_expanded_last:
+  assumes "([S' \<rightarrow> [] \<cdot> [Nt S]], \<gamma> @ [X]) \<turnstile>c* ([A \<rightarrow> [] \<cdot> \<beta>], [])"
+  obtains Y \<delta> \<zeta> where "([S' \<rightarrow> [] \<cdot> [Nt S]], \<gamma> @ [X]) \<turnstile>c* ([Y \<rightarrow> \<delta> @ [X] \<cdot> \<zeta>], [])"
+    "([Y \<rightarrow> \<delta> @ [X] \<cdot> \<zeta>], []) \<turnstile>c* ([A \<rightarrow> [] \<cdot> \<beta>], [])"
+proof -
+  from assms obtain n where "([S' \<rightarrow> [] \<cdot> [Nt S]], \<gamma> @ [X]) \<turnstile>c(n) ([A \<rightarrow> [] \<cdot> \<beta>], [])"
+    using rtranclp_imp_relpowp by fast
+  with that show thesis proof (induction n arbitrary: A \<beta> thesis)
+    case (Suc n)
+    note Suc_n = this
+    then obtain Y \<delta> \<zeta> \<eta> where step: "([S' \<rightarrow> [] \<cdot> [Nt S]], \<gamma> @ [X]) \<turnstile>c(n) ([Y \<rightarrow> \<delta> \<cdot> \<zeta>], \<eta>)"
+      "([Y \<rightarrow> \<delta> \<cdot> \<zeta>], \<eta>) \<turnstile>c ([A \<rightarrow> [] \<cdot> \<beta>], [])"    
+      by (metis item.exhaust relpowp_Suc_E surj_pair)
+    from this(2) show ?case proof cases
+      case (nxt)
+      then show ?thesis using Suc by fast
+    next
+      case (eps)
+      show ?thesis proof (cases n)
+        case 0
+        then show ?thesis using Suc step eps by auto
+      next
+        case (Suc m)
+        show ?thesis proof (cases \<delta> rule: rev_cases)
+          case Nil
+          then show ?thesis using Suc_n step 
+            by (smt (verit, best) eps(1,2) prod.inject rtranclp.rtrancl_into_rtrancl)
+        next
+          case (snoc \<delta>' Z)
+          with Suc step have
+            "([S' \<rightarrow> [] \<cdot> [Nt S]], \<gamma> @ [X]) \<turnstile>c(m) ([Y \<rightarrow> \<delta>' \<cdot> Z # \<zeta>], [Z])"
+            "([Y \<rightarrow> \<delta>' \<cdot> Z # \<zeta>], [Z]) \<turnstile>c ([Y \<rightarrow> \<delta>' @ [Z] \<cdot> \<zeta>], [])" 
+            using char_step_left_nonempty_imp_not_eps char_eps_impossible
+            by (smt (verit, del_insts) Extended_Cfg.char_step_cases Extended_Cfg_axioms 
+                append1_eq_conv eps(1,2) item.inject prod.inject relpowp_Suc_E,
+            use eps(1,4) snoc in force)
+          moreover with char_reachable_imp_substring have "X = Z" 
+            by (metis append1_eq_conv append_assoc relpowp_imp_rtranclp)
+          ultimately show ?thesis using Suc_n(2) snoc step 
+            by (metis Pair_inject eps(1,2) r_into_rtranclp relpowp_imp_rtranclp)
+        qed
+      qed
+    qed
+  qed simp
+qed
 
 section \<open>Equivalences between \<open>char(G)\<close>, \<open>IPDA\<close>, and rightmost derivations\<close>
 
@@ -698,13 +759,13 @@ lemma derivers_imp_ipda:
     "Prods G' \<turnstile> \<beta> \<Rightarrow>* map Tm v"
   obtains \<rho> where 
     "([A \<rightarrow> \<alpha> \<cdot> \<beta>] # \<rho>, v@w) \<turnstile>I* ([I.final_state], [])" 
-    "hist \<rho> = \<gamma>"
+    "hist (rev \<rho>) = \<gamma>"
   using assms(1) proof cases
   case rtrancl_refl
   with assms have eqs: "\<gamma> = [] \<and> w = [] \<and> \<alpha>@\<beta> = [Nt S]" 
     using S'_derive_imp_S append_eq_Cons_conv deriver_imp_derive by fastforce
   then show thesis using S'_derive_imp_S I.deriver_imp_IPDA_comp assms that 
-    by (metis append.right_neutral hist_Nil local.rtrancl_refl map_Tm_Nt_eq_map_Tm_Nt
+    by (metis append.right_neutral hist_Nil local.rtrancl_refl map_Tm_Nt_eq_map_Tm_Nt rev.simps(1)
         self_append_conv2)
 next
   case (rtrancl_into_rtrancl b)
@@ -718,7 +779,7 @@ next
     then have eqs: "\<gamma> = [] \<and> w = [] \<and> \<alpha>@\<beta> = [Nt S] \<and> A = S'" 
       using S'_derive_imp_S append_eq_Cons_conv deriver_imp_derive by fastforce
     then show thesis using S'_derive_imp_S I.deriver_imp_IPDA_comp Nil
-      by (metis append.right_neutral append_Nil hist_Nil list.simps(8))
+      by (metis append.right_neutral hist_Nil list.simps(8) rev.simps(1) self_append_conv2)
   next
     case (Cons i \<rho>)
     then obtain X \<alpha>' \<beta>' where X_defs:
@@ -733,13 +794,13 @@ next
     then obtain \<rho>' where \<rho>'_def:
       "([X \<rightarrow> \<alpha>' @ [Nt A] \<cdot> \<beta>'] # \<rho>', u@v') 
           \<turnstile>I* ([I.final_state], [])"
-      "hist \<rho>' = \<alpha>''" 
+      "hist (rev \<rho>') = \<alpha>''" 
       using Cons(1)[OF X_chain(1) rm_chain_imp_derivers[OF X_chain(1)], of "\<alpha>' @ [Nt A]" \<beta>']
       by (metis append.assoc append_Cons append_Nil derivers_imp_derives)
     from X_defs have X_in_prods: "(X, \<alpha>' @ Nt A # \<beta>') \<in> Prods G'"
       by (metis Cons.prems(1) rm_chain_imp_prod)
     let ?\<rho> = "[X \<rightarrow> \<alpha>' \<cdot> Nt A # \<beta>'] # \<rho>'"
-    have hist_\<rho>: "hist ?\<rho> = \<gamma>" using X_chain(5) \<rho>'_def(2) by simp
+    have hist_\<rho>: "hist (rev ?\<rho>) = \<gamma>" using X_chain(5) \<rho>'_def(2) by simp
     from Cons(4) have A_in_prods: "(A, \<alpha> @ \<beta>) \<in> Prods G'" 
       by (simp add: deriver_imp_in_Prods)
     with I.derives_imp_completes[OF Cons(5)] have 
@@ -814,14 +875,13 @@ text \<open>Step 3: If the configuration \<open>([A \<rightarrow> \<alpha>.\<bet
 
 lemma ipda_imp_char:
   assumes "([A \<rightarrow> \<alpha> \<cdot> \<beta>] # \<rho>, w) \<turnstile>I* ([I.final_state], [])"
-  shows "([S' \<rightarrow> [] \<cdot> [Nt S]], hist \<rho> @ \<alpha>) \<turnstile>c* ([A \<rightarrow> \<alpha> \<cdot> \<beta>], [])"
+  shows "([S' \<rightarrow> [] \<cdot> [Nt S]], hist (rev \<rho>) @ \<alpha>) \<turnstile>c* ([A \<rightarrow> \<alpha> \<cdot> \<beta>], [])"
 using assms proof (induction \<rho> arbitrary: A \<alpha> \<beta> w)
   case Nil
   with I.reaches_without_stack_imp_S' consider (init) "[A \<rightarrow> \<alpha> \<cdot> \<beta>] = [S' \<rightarrow> [] \<cdot> [Nt S]]" | 
     (final) "[A \<rightarrow> \<alpha> \<cdot> \<beta>] = [S' \<rightarrow> [Nt S] \<cdot> []]" by auto
   then show ?case 
-    by cases (metis hist_Cons hist_singleton history_unfold rtranclp.rtrancl_refl,
-    use G'_def char_fa.step.simps hist_singleton in auto)
+    by cases (fastforce simp: G'_def)+
 next
   case (Cons i \<rho>)
   with ipda_reaches_final_imp_rm_chain obtain X \<alpha>' \<beta>' \<gamma> where chain:
@@ -843,10 +903,10 @@ next
     by (metis (no_types, lifting) I.complete_S'_step_impossible I.step_not_expanding_unique
         converse_rtranclpE list.sel(1))
   note X_comp = Cons.IH[OF this]
-  hence "([S' \<rightarrow> [] \<cdot> [Nt S]], hist \<rho> @ \<alpha>') \<turnstile>c* ([X \<rightarrow> \<alpha>' \<cdot> Nt A # \<beta>'], [])"
+  hence "([S' \<rightarrow> [] \<cdot> [Nt S]], hist (rev \<rho>) @ \<alpha>') \<turnstile>c* ([X \<rightarrow> \<alpha>' \<cdot> Nt A # \<beta>'], [])"
     using char_consumes_last_imp_butlast_reaches by fastforce
-  hence "([S' \<rightarrow> [] \<cdot> [Nt S]], hist (i # \<rho>) @ \<alpha>) \<turnstile>c* ([X \<rightarrow> \<alpha>' \<cdot> Nt A # \<beta>'], \<alpha>)"
-    using char_fa.steps_append[of _ "hist (i # \<rho>)" "[]" _ \<alpha>] chain by simp
+  hence "([S' \<rightarrow> [] \<cdot> [Nt S]], hist (rev (i # \<rho>)) @ \<alpha>) \<turnstile>c* ([X \<rightarrow> \<alpha>' \<cdot> Nt A # \<beta>'], \<alpha>)"
+    using char_fa.steps_append[of _ "hist (rev (i # \<rho>))" "[]" _ \<alpha>] chain by simp
   also have "... \<turnstile>c ([A \<rightarrow> [] \<cdot> \<alpha> @ \<beta>], \<alpha>)" 
     using A_in_Prods X_in_Prods by force
   also from this have "... \<turnstile>c* ([A \<rightarrow> \<alpha> \<cdot> \<beta>], [])" 
@@ -878,13 +938,31 @@ inductive reliable_prefix :: "('n, 't) item \<Rightarrow> ('n, 't) syms \<Righta
     Prods G' \<turnstile> \<gamma>' @ Nt A # map Tm w \<Rightarrow>r \<gamma>' @ \<alpha> @ \<beta> @ map Tm w\<rbrakk> 
     \<Longrightarrow> reliable_prefix [A \<rightarrow> \<alpha> \<cdot> \<beta>] (\<gamma>' @ \<alpha>)"
 
-inductive_cases reliable_prefixE: "reliable_prefix [A \<rightarrow> \<alpha> \<cdot> \<beta>] \<gamma>"
+inductive_cases reliable_prefixE [consumes 1]: "reliable_prefix [A \<rightarrow> \<alpha> \<cdot> \<beta>] \<gamma>"
 
 lemma reliable_prefixI [intro]:
   assumes "Prods G' \<turnstile> [Nt S'] \<Rightarrow>r* \<gamma>' @ Nt A # map Tm w"
     "Prods G' \<turnstile> \<gamma>' @ Nt A # map Tm w \<Rightarrow>r \<gamma> @ \<beta> @ map Tm w" "\<gamma> = \<gamma>' @ \<alpha>"
   shows "reliable_prefix [A \<rightarrow> \<alpha> \<cdot> \<beta>] \<gamma>"
   using assms reliable_prefix.intros by auto
+
+lemma reliable_app [simp]:
+  "reliable_prefix [A \<rightarrow> \<alpha> \<cdot> \<beta> @ \<gamma>] \<gamma>' \<Longrightarrow> reliable_prefix [A \<rightarrow> \<alpha> @ \<beta> \<cdot> \<gamma>] (\<gamma>' @ \<beta>)"
+  by (elim reliable_prefixE) auto
+
+lemma reliable_app2 [simp]:
+  "reliable_prefix [A \<rightarrow> \<alpha> @ \<beta> \<cdot> \<gamma>] (\<gamma>' @ \<beta>) \<Longrightarrow> reliable_prefix [A \<rightarrow> \<alpha> \<cdot> \<beta> @ \<gamma>] \<gamma>'"
+  by (elim reliable_prefixE) auto
+
+lemma reliable_imp_in_It:
+  assumes "reliable_prefix [A \<rightarrow> \<alpha> \<cdot> \<beta>] \<gamma>" shows "[A \<rightarrow> \<alpha> \<cdot> \<beta>] \<in> It G'"
+using assms proof (cases rule: reliable_prefixE)
+  case (1 \<gamma>' w)
+  from this(3) have "(A, \<alpha> @ \<beta>) \<in> Prods G'" 
+    by (simp add: deriver_imp_in_Prods)
+  then show ?thesis using in_Prods_imp_in_It by force
+qed
+
 
 text \<open>The words on which \<open>char(G)\<close> reaches \<open>[A \<rightarrow> \<alpha>.\<beta>]\<close> are exactly the reliable 
      prefixes for \<open>[A \<rightarrow> \<alpha>.\<beta>]\<close>:\<close>
@@ -908,16 +986,56 @@ lemma char_fa_init_valid_for_Nil [simp]:
   "reliable_prefix [S' \<rightarrow> [] \<cdot> [Nt S]] []"
   using char_eq_reliable_prefix by fast
 
+lemma char_fa_init_valid_imp_Nil:
+  assumes "reliable_prefix [S' \<rightarrow> [] \<cdot> [Nt S]] \<gamma>"
+  shows "\<gamma> = []"
+  using assms S'_derives_S'_imp_refl derivers_imp_derives 
+  by cases blast
+
+lemma S'_complete_reliable_imp_S:
+  assumes "reliable_prefix [S' \<rightarrow> [Nt S] \<cdot> []] \<gamma>" 
+  shows "\<gamma> = [Nt S]"
+  using assms S'_derives_S'_imp_refl derivers_imp_derives 
+  by cases blast
+
+definition valids :: "('n, 't) syms \<Rightarrow> ('n, 't) item set" where
+  "valids \<gamma> \<equiv> {i. reliable_prefix i \<gamma>}"
+
+lemma validD:
+  "i \<in> valids \<gamma> \<Longrightarrow> reliable_prefix i \<gamma>"
+  unfolding valids_def by simp
+
+lemma validI [intro]:
+  "reliable_prefix i \<gamma> \<Longrightarrow> i \<in> valids \<gamma>"
+  unfolding valids_def by blast
+
 lemma char_fa_nextl_is_valids:
-  "nfa.nextl char_fa (nfa.init char_fa) w = {i. reliable_prefix i w}"
+  "nfa.nextl char_fa (nfa.init char_fa) w = valids w"
 proof -
-  have "{i. reliable_prefix i w} = {i. ([S' \<rightarrow> [] \<cdot> [Nt S]], w) \<turnstile>c* (i, [])}"
-    using char_eq_reliable_prefix by (metis item.exhaust)
+  have "valids w = {i. ([S' \<rightarrow> [] \<cdot> [Nt S]], w) \<turnstile>c* (i, [])}"
+    using char_eq_reliable_prefix unfolding valids_def by (metis item.exhaust)
   also have "... = nfa.nextl char_fa (nfa.init char_fa) w"
     using char_fa.eps_subst_states_imp_nextl_eq_reachable[OF eps_char_fa_subst_states]
     by auto
   finally show ?thesis by order
 qed
+
+lemma eps_reliable_preserved:
+  assumes "(i, k) \<in> (nfa.eps char_fa)\<^sup>*"
+    "reliable_prefix i \<gamma>"
+  shows "reliable_prefix k \<gamma>"
+  using assms proof (induction rule: converse_rtrancl_induct)
+  case (step i j)
+  then obtain A \<alpha> X \<beta> \<delta> where ij_eq: "i = [A \<rightarrow> \<alpha> \<cdot> Nt X # \<beta>]" "j = [X \<rightarrow> [] \<cdot> \<delta>]"
+    by blast
+  from step(4) show ?case unfolding ij_eq proof cases
+    case (1 \<gamma>' w)
+    hence "reliable_prefix j \<gamma>" using ij_eq 
+      by (metis (no_types, lifting) char_eq_reliable_prefix char_fa.step_eps
+          rtranclp.rtrancl_into_rtrancl step.hyps(1) step.prems)
+    then show ?thesis using step by argo
+  qed
+qed satx
 
 lemma derivern_Suc_imp_reliable:
   assumes "Prods G' \<turnstile> [Nt S'] \<Rightarrow>r(Suc n) \<alpha> @ Nt X # map Tm w"
@@ -961,9 +1079,9 @@ proof -
     from Cons(3) show ?case proof cases
       case (step \<alpha>' A v \<alpha>'' Y \<beta>' u)
       note i_step = this
-      hence eqs [simp]: "\<alpha>' @ \<alpha>'' = \<alpha> @ \<beta> \<and> Y = X \<and> u @ v = w"
-        by (metis Cons.prems(2) append.assoc append_eq_map_conv hist_Cons history_unfold list.inject
-            map_Tm_inject_iff rm_chain_singleton_left_is_hist same_append_eq sym.inject(1))
+      from this(2) have eqs [simp]: "\<alpha>' @ \<alpha>'' = \<alpha> @ \<beta> \<and> Y = X \<and> u @ v = w"
+        using rm_eq_imp_eq[of "\<alpha> @ \<beta>" X w "\<alpha>' @ \<alpha>''" Y "u @ v"]  
+        by (metis append_eq_appendI map_append)
       from step(3) show ?thesis proof cases
         case refl
         with eqs i_step have is_S: "\<alpha> @ \<beta> @ Nt Y # \<beta>' @ map Tm v = [Nt S] \<and> \<alpha> = []"
@@ -1087,6 +1205,20 @@ lemma states_dfa_LR0 [simp]:
   "dfa.states LR\<^sub>0 = dfa.accessible char_fa.Power_dfa"
   unfolding LR\<^sub>0_def by (simp add: char_fa.dfa_Power dfa.states_Accessible_dfa)
 
+lemma init_dfa_LR0 [simp]:
+  "dfa.init LR\<^sub>0 = {q. ([S' \<rightarrow> [] \<cdot> [Nt S]], q) \<in> (nfa.eps char_fa)\<^sup>*}"
+proof -
+  have "dfa.init LR\<^sub>0 = char_fa.epsclo {[S' \<rightarrow> [] \<cdot> [Nt S]]}"
+    by (simp add: LR\<^sub>0_def char_fa.dfa_Power dfa.init_Accessible_dfa)
+  also have "... = nfa.states char_fa \<inter> {q. ([S' \<rightarrow> [] \<cdot> [Nt S]], q) \<in> (nfa.eps char_fa)\<^sup>*}"
+    unfolding char_fa.epsclo_def by fast
+  also have "... = {q. ([S' \<rightarrow> [] \<cdot> [Nt S]], q) \<in> (nfa.eps char_fa)\<^sup>*}"
+    by (standard, simp, standard, standard)
+    (use in_eps_char_star_imp_in_It states_char_fa char_fa.init init_char_fa 
+      in blast)+
+  finally show ?thesis .
+qed
+    
 
 lemma dfa_LR0_states_subset [dest]:
   "q \<in> dfa.states LR\<^sub>0 \<Longrightarrow> q \<in> dfa.states char_fa.Power_dfa"
@@ -1134,15 +1266,11 @@ lemma in_state_imp_in_It:
   shows "i \<in> It G'"
   using assms states_dfa_LR0 states_char_fa char_fa.epsclo_subset by fastforce
 
-lemma nxt_LR0_eq_intersect:
-  "dfa.nxt LR\<^sub>0 Q a = dfa.nxt LR\<^sub>0 (Q \<inter> It G') a"
-  unfolding LR\<^sub>0_def by (simp add: char_fa.dfa_Power dfa.nxt_Accessible_dfa)
-
 lemma finite_dfa_LR0_nempty_syms:
   "finite {a. dfa.nxt LR\<^sub>0 q a \<noteq> {}}"
 proof -
   have "{a. dfa.nxt LR\<^sub>0 q a \<noteq> {}} = {a. dfa.nxt LR\<^sub>0 (q \<inter> It G') a \<noteq> {}}"
-    using nxt_LR0_eq_intersect by presburger
+    by simp
   moreover have "... \<subseteq> (\<lambda>i. case i of [X \<rightarrow> \<alpha> \<cdot> Y # \<beta>] \<Rightarrow> Y) ` char_fa.epsclo (q \<inter> It G')"
     (is "?A \<subseteq> ?f ` ?Q'")
   proof 
@@ -1166,18 +1294,155 @@ proof -
 qed
 
 lemma nextl_dfa_LR0_is_valids:
-  "dfa.nextl LR\<^sub>0 (dfa.init LR\<^sub>0) \<gamma> = {i. reliable_prefix i \<gamma>}"
+  "dfa.nextl LR\<^sub>0 (dfa.init LR\<^sub>0) \<gamma> = valids \<gamma>"
   using LR\<^sub>0_def char_fa.Power_nextl_eq_nfa_nextl char_fa_nextl_is_valids 
    dfa_LR0_nextl by presburger
 
 lemma state_imp_valids:
-  "p \<in> dfa.states LR\<^sub>0 \<Longrightarrow> \<exists>\<gamma>. p = {i. reliable_prefix i \<gamma>}"
+  "p \<in> dfa.states LR\<^sub>0 \<Longrightarrow> \<exists>\<gamma>. p = valids \<gamma>"
   using nextl_dfa_LR0_is_valids dfa.path_to_left_lang[OF char_fa.dfa_Power]
-    dfa.nextl_path_to[OF char_fa.dfa_Power] by fastforce
+    dfa.nextl_path_to[OF char_fa.dfa_Power] by (metis dfa_LR0_nextl states_dfa_LR0)
+
+lemma dfa_LR0_nxt_is_epsclo_of_shift:
+  assumes "Q \<in> dfa.states LR\<^sub>0"
+  shows "dfa.nxt LR\<^sub>0 Q Y = char_fa.epsclo {[X \<rightarrow> \<alpha> @ [Y] \<cdot> \<beta>]|X \<alpha> \<beta>. [X \<rightarrow> \<alpha> \<cdot> Y # \<beta>] \<in> Q}"
+proof -
+  from dfa_LR0_states_subset[OF assms(1)] char_fa.epsclo_idem
+  have "dfa.nxt LR\<^sub>0 Q Y = (\<Union>i \<in> Q. char_fa.epsclo (nfa.nxt char_fa i Y))"
+    unfolding dfa_LR0_nxt char_fa.nxt_Power_dfa char_fa.states_Power_dfa by blast
+  also have "... = char_fa.epsclo (\<Union>i \<in> Q. (nfa.nxt char_fa i Y))"
+    by auto
+  finally show ?thesis using char_fa_nxts_is_shifts 
+    by (metis (lifting) assms in_state_imp_in_It subsetI)
+qed
+
+
+lemma nxt_dfa_LR0_shift_is_valids_app:
+  assumes "valids \<gamma> \<in> dfa.states LR\<^sub>0"
+  shows "dfa.nxt LR\<^sub>0 (valids \<gamma>) X = valids (\<gamma> @ [X])"
+proof (simp only: dfa_LR0_nxt_is_epsclo_of_shift[OF assms], standard)
+  show " char_fa.epsclo {[Xa \<rightarrow> \<alpha> @ [X] \<cdot> \<beta>] |Xa \<alpha> \<beta>. [Xa \<rightarrow> \<alpha> \<cdot> X # \<beta>] \<in> valids \<gamma>} 
+    \<subseteq> valids (\<gamma> @ [X])" (is "?\<delta> \<subseteq> _")
+  proof
+    fix i
+    assume "i \<in> ?\<delta>" 
+    then obtain Y \<alpha> \<beta> where "[Y \<rightarrow> \<alpha> \<cdot> X # \<beta>] \<in> valids \<gamma>" 
+      "([Y \<rightarrow> \<alpha> @ [X] \<cdot> \<beta>], i) \<in> (nfa.eps char_fa)\<^sup>*"
+      unfolding char_fa.epsclo_def using assms by blast
+    moreover from validD[OF this(1)] have "reliable_prefix [Y \<rightarrow> \<alpha> @ [X] \<cdot> \<beta>] (\<gamma> @ [X])"
+      by cases auto
+    ultimately show "i \<in> valids (\<gamma> @ [X])"
+      by (intro validI) (use eps_reliable_preserved in blast)
+  qed
+  show "valids (\<gamma> @ [X]) \<subseteq> ?\<delta>"
+  proof 
+    fix i
+    assume i_valid: "i \<in> valids (\<gamma> @ [X])"
+    consider (noncomp) A \<alpha> \<beta> where "i = [A \<rightarrow> \<alpha> @ [X] \<cdot> \<beta>]" |(complete) A \<beta> where "i = [A \<rightarrow> [] \<cdot> \<beta>]"
+    proof -
+      obtain A \<alpha> \<beta> where i_A: "i = [A \<rightarrow> \<alpha> \<cdot> \<beta>]" using item.exhaust by blast
+      show thesis proof (cases \<alpha> rule: rev_cases)
+        case (snoc \<alpha>' Y)
+        then show ?thesis using i_A i_valid validD that(1) 
+          by (metis append.assoc append1_eq_conv reliable_prefixE)
+      qed (use that i_A in blast)
+    qed
+    then show "i \<in> ?\<delta>" proof cases
+      case noncomp
+      with i_valid[THEN validD] have "reliable_prefix [A \<rightarrow> \<alpha> \<cdot> X # \<beta>] \<gamma>"
+        by (fastforce elim: reliable_prefixE)
+      then show ?thesis using noncomp char_fa.in_states_imp_in_epsclo reliable_imp_in_It
+        by (metis (mono_tags, lifting) \<open>reliable_prefix i (\<gamma> @ [X])\<close> 
+            mem_Collect_eq states_char_fa validI)
+    next
+      case complete
+      from i_valid[THEN validD] obtain Y \<delta> \<zeta> where 
+        "([S' \<rightarrow> [] \<cdot> [Nt S]], \<gamma> @ [X]) \<turnstile>c* ([Y \<rightarrow> \<delta> @ [X] \<cdot> \<zeta>], [])"
+        "([Y \<rightarrow> \<delta> @ [X] \<cdot> \<zeta>], []) \<turnstile>c* (i, [])"
+        unfolding complete using char_eq_reliable_prefix char_reaches_left_empty_imp_expanded_last
+        by blast
+      moreover then have "reliable_prefix [Y \<rightarrow> \<delta> \<cdot> X # \<zeta>] \<gamma>"   
+        by (metis append_Cons append_Nil char_eq_reliable_prefix reliable_app2)
+      moreover from calculation(2) have "([Y \<rightarrow> \<delta> @ [X] \<cdot> \<zeta>], i) \<in> (nfa.eps char_fa)\<^sup>*"
+        using char_steps_unchanged_imp_in_eps_star by blast
+      ultimately show ?thesis unfolding char_fa.epsclo_def 
+        using \<open>reliable_prefix i (\<gamma> @ [X])\<close> complete reliable_imp_in_It by fastforce
+    qed
+  qed
+qed
+
+lemma nxt_dfa_LR0_nempty_imp_ex_shift:
+  assumes "Q \<in> dfa.states LR\<^sub>0" "dfa.nxt LR\<^sub>0 Q Y \<noteq> {}"
+  obtains X \<alpha> \<beta> where "[X \<rightarrow> \<alpha> \<cdot> Y # \<beta>] \<in> Q" "[X \<rightarrow> \<alpha> @ [Y] \<cdot> \<beta>] \<in> dfa.nxt LR\<^sub>0 Q Y"
+proof -
+  from dfa_LR0_nxt_is_epsclo_of_shift[OF assms(1)] assms(2) obtain X \<alpha> \<beta> where
+    "[X \<rightarrow> \<alpha> \<cdot> Y # \<beta>] \<in> Q" by fastforce
+  moreover from this assms in_state_imp_in_It have "[X \<rightarrow> \<alpha> \<cdot> Y # \<beta>] \<in> nfa.states char_fa" 
+    by auto
+  moreover from this have "[X \<rightarrow> \<alpha> @ [Y] \<cdot> \<beta>] \<in> nfa.states char_fa"  
+    using char_fa.nxt in_It_imp_in_Prods by fastforce
+  moreover have "([X \<rightarrow> \<alpha> @ [Y] \<cdot> \<beta>], [X \<rightarrow> \<alpha> @ [Y] \<cdot> \<beta>]) \<in> (nfa.eps char_fa)\<^sup>*" by blast
+  ultimately show thesis using that dfa_LR0_nxt_is_epsclo_of_shift[OF assms(1)] 
+    unfolding char_fa.epsclo_def by blast
+qed
+
+lemma in_nxt_dfa_LR0_imp_shift_or_left_empty:
+  assumes "Q \<in> dfa.states LR\<^sub>0" "i \<in> dfa.nxt LR\<^sub>0 Q X"
+  obtains A \<alpha> where "i = [A \<rightarrow> [] \<cdot> \<alpha>]" |
+    A \<alpha> \<beta> where "i = [A \<rightarrow> \<alpha> @ [X] \<cdot> \<beta>]"
+proof -
+  note nxt_shifts = dfa_LR0_nxt_is_epsclo_of_shift[OF assms(1), of X]
+  from assms obtain A \<alpha> \<beta> where eps: "[A \<rightarrow> \<alpha> \<cdot> X # \<beta>] \<in> Q" 
+    "([A \<rightarrow> \<alpha> @ [X] \<cdot> \<beta>], i) \<in> (nfa.eps char_fa)\<^sup>*"
+    unfolding nxt_shifts char_fa.epsclo_def by fast
+  from eps(2) show thesis by cases (use that in blast)+
+qed
+    
+lemma dfa_LR0_nxt_final_impossible:
+  assumes "p \<in> dfa.states LR\<^sub>0"
+  shows "dfa.nxt LR\<^sub>0 p X = {[S' \<rightarrow> [] \<cdot> []]} \<Longrightarrow> False"
+proof (simp only: dfa_LR0_nxt_is_epsclo_of_shift[OF assms])
+  let ?q = "char_fa.epsclo {[Xa \<rightarrow> \<alpha> @ [X] \<cdot> \<beta>] |Xa \<alpha> \<beta>. [Xa \<rightarrow> \<alpha> \<cdot> X # \<beta>] \<in> p}"
+  assume eq: "?q = {[S' \<rightarrow> [] \<cdot> []]}"
+  show False
+  proof (cases "?q = {}")
+    case False
+    then obtain Y \<alpha> \<beta> where "[Y \<rightarrow> \<alpha> @ [X] \<cdot> \<beta>] \<in> ?q" using char_fa.in_states_imp_in_epsclo
+        assms in_state_imp_in_It
+      by (smt (verit, del_insts) S'_derive_imp_S S'_derives_S'_imp_refl append_self_conv2
+          char_fa.epsclo_subset deriver_imp_derive derivers_imp_derives eq in_states_imp_valid
+          insert_subset item.inject list.distinct(1) reliable_prefix.simps)
+    then show ?thesis using eq by auto
+  qed (use eq in simp)
+qed
+
+lemma inj_nxt_dfa_LR0_if_nempty:
+  assumes "q \<in> dfa.states LR\<^sub>0" "dfa.nxt LR\<^sub>0 q X = dfa.nxt LR\<^sub>0 q Y"
+    "dfa.nxt LR\<^sub>0 q X \<noteq> {}"
+  shows "X = Y"
+proof -
+  obtain A \<alpha> \<beta> where "[A \<rightarrow> \<alpha> @ [X] \<cdot> \<beta>] \<in> dfa.nxt LR\<^sub>0 q X" "[A \<rightarrow> \<alpha> \<cdot> X # \<beta>] \<in> q"
+    using nxt_dfa_LR0_nempty_imp_ex_shift assms by metis
+  moreover from this have "[A \<rightarrow> \<alpha> @ [X] \<cdot> \<beta>] \<in> dfa.nxt LR\<^sub>0 q Y"
+    using assms by argo
+  ultimately show ?thesis using in_nxt_dfa_LR0_imp_shift_or_left_empty
+      dfa_LR0.nxt assms by blast
+qed
+
+
+lemma dfa_LR0_init_reliable_Nil:
+  assumes "dfa.init LR\<^sub>0 = valids \<gamma>"
+  shows "\<gamma> = []"
+proof -
+  from assms have "reliable_prefix [S' \<rightarrow> [] \<cdot> [Nt S]] \<gamma>"   
+    by (metis char_fa_init_valid_for_Nil dfa_LR0.nextl.simps(1) mem_Collect_eq
+        nextl_dfa_LR0_is_valids valids_def)
+  with char_fa_init_valid_imp_Nil show ?thesis by simp
+qed
 
 section \<open>The Canonical LR(0) Parser\<close>
 
-definition P\<^sub>0 :: "(('n, 't) item set, 't) npda" where
+definition P\<^sub>0 :: "(('n, 't) item set, 't) gpda" where
   "P\<^sub>0 \<equiv> let 
   \<Delta>\<^sub>G = dfa.nxt LR\<^sub>0;
   q\<^sub>0 = dfa.init LR\<^sub>0;
@@ -1187,45 +1452,90 @@ definition P\<^sub>0 :: "(('n, 't) item set, 't) npda" where
   \<E> = {let q = last (q\<^sub>n#qs) in (q\<^sub>n # qs, \<Delta>\<^sub>G q (Nt X) # [q])| 
        q\<^sub>n qs X \<alpha>. set (q\<^sub>n#qs) \<subseteq> Q \<and> [X \<rightarrow> \<alpha> \<cdot> []] \<in> q\<^sub>n \<and> length \<alpha> = length qs \<and> X \<noteq> S'} \<union>
       {([q, q\<^sub>0], [f])|q. q \<in> Q \<and> [S' \<rightarrow> [Nt S] \<cdot> []] \<in> q}
- in \<lparr>npda.states = Q \<union> {f}, init = q\<^sub>0, final = {f}, nxt = \<Delta>\<^sub>0, eps = \<E>\<rparr>"
+ in \<lparr>gpda.states = Q \<union> {f}, init = q\<^sub>0, final = {f}, nxt = \<Delta>\<^sub>0, eps = \<E>\<rparr>"
 
 lemma states_P0: 
-  "npda.states P\<^sub>0 = dfa.states LR\<^sub>0 \<union> {{[S' \<rightarrow> [] \<cdot> []]}}"
-  unfolding P\<^sub>0_def by (meson npda.select_convs(1))
+  "gpda.states P\<^sub>0 = dfa.states LR\<^sub>0 \<union> {{[S' \<rightarrow> [] \<cdot> []]}}"
+  unfolding P\<^sub>0_def by (meson gpda.select_convs(1))
 
 lemma init_P0: 
-  "npda.init P\<^sub>0 = dfa.init LR\<^sub>0"
-  unfolding P\<^sub>0_def by (meson npda.select_convs(2))
+  "gpda.init P\<^sub>0 = dfa.init LR\<^sub>0"
+  unfolding P\<^sub>0_def by (meson gpda.select_convs(2))
+
+lemma init_P0_is_valids_empty:
+  "gpda.init P\<^sub>0 = {i. reliable_prefix i []}"
+  by (metis dfa_LR0.nextl.simps(1) init_P0 nextl_dfa_LR0_is_valids valids_def)
+
 
 abbreviation "P0_final \<equiv> {[S' \<rightarrow> [] \<cdot> []]}"
 
-lemma final_P0:
-  "npda.final P\<^sub>0 = {P0_final}"
-  unfolding P\<^sub>0_def by (meson npda.select_convs(3))
+lemma final_P0 [simp]:
+  "gpda.final P\<^sub>0 = {P0_final}"
+  unfolding P\<^sub>0_def by (meson gpda.select_convs(3))
+
+lemma init_P0_contains_S'S [simp]:
+  "[S' \<rightarrow> [] \<cdot> [Nt S]] \<in> gpda.init P\<^sub>0"
+  unfolding init_P0 init_dfa_LR0 
+  using char_fa.epsclo_increasing char_fa.init by auto
+
+lemma P0_init_not_final [simp]:
+  "gpda.init P\<^sub>0 \<notin> gpda.final P\<^sub>0"
+  unfolding final_P0 init_dfa_LR0 using init_P0_contains_S'S by fast
+
+
+lemma P0_final_item_notin_It [simp]:
+  "[S' \<rightarrow> [] \<cdot> []] \<notin> It G'"
+  using Extended_Cfg.S'_Prod_notin_G(1) Extended_Cfg_axioms G'_def in_It_imp_in_Prods
+  by fastforce
+
+lemma dfa_LR0_nxt_final_impossible_P0:
+  assumes "p \<in> gpda.states P\<^sub>0"
+  shows "dfa.nxt LR\<^sub>0 p X = {[S' \<rightarrow> [] \<cdot> []]} \<Longrightarrow> False"
+proof -
+  assume eq: "dfa.nxt LR\<^sub>0 p X = {[S' \<rightarrow> [] \<cdot> []]}"
+  from assms consider "p \<in> dfa.states LR\<^sub>0" | "p = {[S' \<rightarrow> [] \<cdot> []]}"
+    using states_P0 by blast
+  thus False proof cases
+    case 1
+    then show ?thesis using dfa_LR0_nxt_final_impossible eq by presburger 
+  next
+    case 2
+    hence no_states: "p \<inter> nfa.states char_fa = {}" using P0_final_item_notin_It
+      by simp
+    hence epsclo_empty: "char_fa.epsclo p = {}" unfolding char_fa.epsclo_def 
+      by (metis char_fa.epsclo_def char_fa.epsclo_empty char_fa_epsclo_It_intersect_eq
+          states_char_fa)
+    have "dfa.nxt LR\<^sub>0 p X = (\<Union>i \<in> char_fa.epsclo p. char_fa.epsclo (nfa.nxt char_fa i X))"
+      by auto
+    also from no_states epsclo_empty have "... = {}"
+      by blast
+    finally show ?thesis using eq by blast
+  qed
+qed
 
 lemma nxt_P0:
-  "npda.nxt P\<^sub>0 = 
+  "gpda.nxt P\<^sub>0 = 
     {([q], a, dfa.nxt LR\<^sub>0 q (Tm a) # [q])|q a. q \<in> dfa.states LR\<^sub>0 \<and> dfa.nxt LR\<^sub>0 q (Tm a) \<noteq> {}}"
-  unfolding P\<^sub>0_def by (meson npda.select_convs(4))
+  unfolding P\<^sub>0_def by (meson gpda.select_convs(4))
 
 lemma eps_P0:
-  "npda.eps P\<^sub>0 = 
+  "gpda.eps P\<^sub>0 = 
   {let q = last (q\<^sub>n#qs) in (q\<^sub>n # qs, dfa.nxt LR\<^sub>0 q (Nt X) # [q])|
     q\<^sub>n qs X \<alpha>. set (q\<^sub>n#qs) \<subseteq> dfa.states LR\<^sub>0 \<and> [X \<rightarrow> \<alpha> \<cdot> []] \<in> q\<^sub>n \<and> length \<alpha> = length qs \<and> X \<noteq> S'} \<union>
   {([q, dfa.init LR\<^sub>0], [P0_final])|q. q \<in> dfa.states LR\<^sub>0 \<and> [S' \<rightarrow> [Nt S] \<cdot> []] \<in> q}"
-  unfolding P\<^sub>0_def by (meson npda.select_convs(5))
+  unfolding P\<^sub>0_def by (meson gpda.select_convs(5))
 
 lemmas P\<^sub>0_simps [simp] = states_P0 init_P0 final_P0 nxt_P0 eps_P0
 
 lemma nxt_P0E [elim]:
-  assumes "(qs, a, qs') \<in> npda.nxt P\<^sub>0"
+  assumes "(qs, a, qs') \<in> gpda.nxt P\<^sub>0"
   obtains q where "qs = [q]" "qs' = dfa.nxt LR\<^sub>0 q (Tm a) # [q]"
     "q \<in> dfa.states LR\<^sub>0" "dfa.nxt LR\<^sub>0 q (Tm a) \<noteq> {}"
   using assms by auto
 
 
 lemma eps_P0E [elim, consumes 1, case_names reduce finish]:
-  assumes "(ps, qs) \<in> npda.eps P\<^sub>0"
+  assumes "(ps, qs) \<in> gpda.eps P\<^sub>0"
   obtains 
     p ps' X \<alpha> where "ps = p # ps'" "qs = [dfa.nxt LR\<^sub>0 (last ps) (Nt X), last ps]"
     "set ps \<subseteq> dfa.states LR\<^sub>0" "[X \<rightarrow> \<alpha> \<cdot> []] \<in> p" "length \<alpha> = length ps'" "X \<noteq> S'"  |
@@ -1314,14 +1624,14 @@ proof (rule finite_surj)
 qed (rule dfa_LR0.finite)
 
 lemma eps_P0_cases[consumes 1, case_names reduce finish]:
-  assumes "(ps, qs) \<in> npda.eps P\<^sub>0"
+  assumes "(ps, qs) \<in> gpda.eps P\<^sub>0"
   obtains r rs X \<alpha> where 
     "ps = r # rs" "qs = (let q = last (r # rs) in dfa.nxt LR\<^sub>0 q (Nt X) # [q])"
     "set (r # rs) \<subseteq> dfa.states LR\<^sub>0" "[X \<rightarrow> \<alpha> \<cdot> []] \<in> r" "length \<alpha> = length rs" |
     q where "q \<in> dfa.states LR\<^sub>0" "ps = [q, dfa.init LR\<^sub>0]" "qs = [P0_final]"
   using assms unfolding eps_P0 by standard (smt (verit, best) mem_Collect_eq prod.inject)+
 
-interpretation P0: npda P\<^sub>0
+interpretation P0: gpda P\<^sub>0
 proof (unfold_locales, goal_cases _ _ nxt eps _ finite_nxt finite_eps)
   case (nxt ps a qs)
   with nxt_P0E obtain p where "ps = [p]"
@@ -1333,11 +1643,11 @@ next
   then show ?case 
   proof (cases rule: eps_P0_cases, intro conjI)
     case (reduce r rs X \<alpha>)
-    then show "qs \<noteq> []" "set ps \<subseteq> npda.states P\<^sub>0" and ps_Cons: "ps \<noteq> []"
+    then show "qs \<noteq> []" "set ps \<subseteq> gpda.states P\<^sub>0" and ps_Cons: "ps \<noteq> []"
       by (metis list.distinct(1), auto)
     from reduce(3) have "dfa.nxt LR\<^sub>0 (last (r # rs)) (Nt X) \<in> dfa.states LR\<^sub>0"
       using dfa_LR0.nxt last_in_set by blast
-    with reduce(1-3) ps_Cons show "set qs \<subseteq> npda.states P\<^sub>0" 
+    with reduce(1-3) ps_Cons show "set qs \<subseteq> gpda.states P\<^sub>0" 
       by (metis (no_types, lifting) Un_iff empty_set insert_subset last_in_set list.simps(15) 
           states_P0 subset_code(1))
   qed (use dfa_LR0.init in simp)
@@ -1349,24 +1659,24 @@ next
       by blast
     with finite_dfa_LR0_nempty_Tms dfa_LR0.finite show ?thesis by auto
   qed
-  moreover have "bij_betw (\<lambda>(q, a). ([q], a, dfa.nxt LR\<^sub>0 q (Tm a) # [q])) ?R (npda.nxt P\<^sub>0)"
+  moreover have "bij_betw (\<lambda>(q, a). ([q], a, dfa.nxt LR\<^sub>0 q (Tm a) # [q])) ?R (gpda.nxt P\<^sub>0)"
     (is "bij_betw ?f _ _")
   proof -
     have "inj_on ?f ?R" by standard auto
-  moreover have "?f ` ?R = (npda.nxt P\<^sub>0)" unfolding nxt_P0 by fastforce
+  moreover have "?f ` ?R = (gpda.nxt P\<^sub>0)" unfolding nxt_P0 by fastforce
   ultimately show ?thesis unfolding bij_betw_def by satx
   qed
   ultimately show ?case using bij_betw_finite by blast
 next
   case finite_eps
-  then show ?case using finite_eps_P0_reduce finite_eps_P0_finish sorry
+  then show ?case using finite_eps_P0_reduce finite_eps_P0_finish by fastforce
 qed (use dfa_LR0.init dfa_LR0.finite in simp_all)
 
 lemma P0_read_iff_in_q:
-"([q], a, dfa.nxt LR\<^sub>0 q (Tm a) # [q]) \<in> npda.nxt P\<^sub>0 
+"([q], a, dfa.nxt LR\<^sub>0 q (Tm a) # [q]) \<in> gpda.nxt P\<^sub>0 
   = (\<exists>X \<alpha> \<beta>. [X \<rightarrow> \<alpha> \<cdot> Tm a # \<beta>] \<in> q \<and> q \<in> dfa.states LR\<^sub>0)"
 proof 
-  assume "([q], a, dfa.nxt LR\<^sub>0 q (Tm a) # [q]) \<in> npda.nxt P\<^sub>0"
+  assume "([q], a, dfa.nxt LR\<^sub>0 q (Tm a) # [q]) \<in> gpda.nxt P\<^sub>0"
   with nxt_P0 have q_nxt: "q \<in> dfa.states LR\<^sub>0" "dfa.nxt LR\<^sub>0 q (Tm a) \<noteq> {}" by auto
   with char_fa.nxt_Power_dfa obtain i where i_defs:
     "i \<in> char_fa.epsclo q" "char_fa.epsclo (nfa.nxt char_fa i (Tm a)) \<noteq> {}"
@@ -1390,14 +1700,14 @@ next
   ultimately have "char_fa.epsclo (nfa.nxt char_fa [X \<rightarrow> \<alpha> \<cdot> Tm a # \<beta>] (Tm a)) \<noteq> {}" 
     using char_fa.epsclo_increasing char_fa.nxt by fast
   hence "dfa.nxt LR\<^sub>0 q (Tm a) \<noteq> {}" using X_epsclo by fastforce
-  thus "([q], a, dfa.nxt LR\<^sub>0 q (Tm a) # [q]) \<in> npda.nxt P\<^sub>0" using nxt_P0 q_state by blast
+  thus "([q], a, dfa.nxt LR\<^sub>0 q (Tm a) # [q]) \<in> gpda.nxt P\<^sub>0" using nxt_P0 q_state by blast
 qed
 
 lemma P0_complete_imp_reduce:
   assumes "[X \<rightarrow> \<alpha> \<cdot> []] \<in> q"
     "X \<noteq> S'"
     "q \<in> dfa.states LR\<^sub>0"
-  obtains qs where "(q#qs, [dfa.nxt LR\<^sub>0 (last (q#qs)) (Nt X), last (q#qs)]) \<in> npda.eps P\<^sub>0"
+  obtains qs where "(q#qs, [dfa.nxt LR\<^sub>0 (last (q#qs)) (Nt X), last (q#qs)]) \<in> gpda.eps P\<^sub>0"
     "length qs = length \<alpha>"
 proof -
   obtain qs where "set qs \<subseteq> dfa.states LR\<^sub>0" "length qs = length \<alpha>"
@@ -1410,7 +1720,7 @@ qed
 
 lemma P0_completes_nempty_imp_eps:
   assumes "completes p \<noteq> {}" "p \<in> dfa.states LR\<^sub>0"
-  obtains ps qs where "(p#ps, qs) \<in> npda.eps P\<^sub>0"
+  obtains ps qs where "(p#ps, qs) \<in> gpda.eps P\<^sub>0"
 proof -
   from assms obtain X \<alpha> where X_def: "[X \<rightarrow> \<alpha> \<cdot> []] \<in> p" by blast
   thus thesis proof (cases "X = S'")
@@ -1432,7 +1742,7 @@ notation P0.stepn (\<open>_ \<turnstile>P'(_') _\<close> 55)
 section \<open>LR(0)-Adequate and Inadequate States\<close>
 
 inductive shift_reduce :: "('n, 't) item set \<Rightarrow> bool" where
-  "\<lbrakk>([p], a, ps) \<in> npda.nxt P\<^sub>0; (p#ps', qs) \<in> npda.eps P\<^sub>0\<rbrakk> \<Longrightarrow> shift_reduce p"
+  "\<lbrakk>([p], a, ps) \<in> gpda.nxt P\<^sub>0; (p#ps', qs) \<in> gpda.eps P\<^sub>0\<rbrakk> \<Longrightarrow> shift_reduce p"
 
 lemma shift_reduceE [elim]:
   assumes "shift_reduce q"
@@ -1470,17 +1780,17 @@ lemma complete_noncomplete_Tm_imp_inadequate:
   assumes "completes q \<noteq> {}" "[X \<rightarrow> \<alpha> \<cdot> Tm a # \<beta>] \<in> q" "q \<in> dfa.states LR\<^sub>0"
   shows "LR0_inadequate q"
 proof -
-  from assms P0_read_iff_in_q have nxt: "([q], a, [dfa.nxt LR\<^sub>0 q (Tm a), q]) \<in> npda.nxt P\<^sub>0" 
+  from assms P0_read_iff_in_q have nxt: "([q], a, [dfa.nxt LR\<^sub>0 q (Tm a), q]) \<in> gpda.nxt P\<^sub>0" 
     by metis
   moreover from assms P0_completes_nempty_imp_eps[OF assms(1,3)] 
-  obtain qs rs where "(q#qs, rs) \<in> npda.eps P\<^sub>0" by blast
+  obtain qs rs where "(q#qs, rs) \<in> gpda.eps P\<^sub>0" by blast
   ultimately show ?thesis unfolding LR0_inadequate_def using shift_reduce.intros by blast
 qed
 
 
 lemma LR0_adequate_complete_cases[consumes 2, case_names empty singleton]:
   assumes "LR0_adequate q"
-    "q \<in> npda.states P\<^sub>0"
+    "q \<in> gpda.states P\<^sub>0"
   obtains "completes q = {}" |
     A \<alpha> where "completes q = {[A \<rightarrow> \<alpha> \<cdot> []]}"
 proof -
@@ -1506,7 +1816,7 @@ qed
 lemma complete_in_adequate_imp_singleton:
   assumes "i \<in> completes q"
     "LR0_adequate q"
-    "q \<in> npda.states P\<^sub>0"
+    "q \<in> gpda.states P\<^sub>0"
   shows "completes q = {i}"
   using assms(2-) by (cases rule: LR0_adequate_complete_cases) (use assms in auto)
 
@@ -1678,7 +1988,7 @@ qed
 lemma LR0_adequate_cases[consumes 2, case_names completes_empty singleton comp_unique, 
       cases set: LR0_adequate]:
   assumes "LR0_adequate q"
-    "q \<in> npda.states P\<^sub>0"
+    "q \<in> gpda.states P\<^sub>0"
   obtains "completes q = {}" |
     A \<alpha> where "q = {[A \<rightarrow> \<alpha> \<cdot> []]}" |
       A where "completes q = {[A \<rightarrow> [] \<cdot> []]}" 
@@ -1734,7 +2044,8 @@ proof
   assume LR0: "is_LR 0"
   from assms(2) obtain X \<beta> Y \<delta> a \<alpha> where "[X \<rightarrow> \<beta> \<cdot> []] \<in> q" "[Y \<rightarrow> \<delta> \<cdot> Tm a # \<alpha>] \<in> q" by fast 
   then obtain \<gamma> where "reliable_prefix ([X \<rightarrow> \<beta> \<cdot> []]) \<gamma>"
-    "reliable_prefix [Y \<rightarrow> \<delta> \<cdot> Tm a # \<alpha>] \<gamma>" using state_imp_valids assms(1) by auto
+    "reliable_prefix [Y \<rightarrow> \<delta> \<cdot> Tm a # \<alpha>] \<gamma>" using state_imp_valids assms(1) 
+    by (blast dest: validD)
   then obtain \<gamma>' w \<nu> y where X_reliable:
     "Prods G' \<turnstile> [Nt S'] \<Rightarrow>r* \<gamma>' @ Nt X # map Tm w"
     "Prods G' \<turnstile>  \<gamma>' @ Nt X # map Tm w \<Rightarrow>r \<gamma>' @ \<beta> @ map Tm w" 
@@ -1784,17 +2095,18 @@ qed
 
 lemma is_LR0_imp_no_LR0_inadequate_states:
   assumes LR0: "is_LR 0"
-  shows "\<forall>q\<in>npda.states P\<^sub>0. LR0_adequate q"
+  shows "\<forall>q\<in>gpda.states P\<^sub>0. LR0_adequate q"
 proof (rule ccontr)
-  assume "\<not>(\<forall>q\<in>npda.states P\<^sub>0. LR0_adequate q)"
-  then obtain q where q_inadequate: "q \<in> npda.states P\<^sub>0" "LR0_inadequate q" by blast
+  assume "\<not>(\<forall>q\<in>gpda.states P\<^sub>0. LR0_adequate q)"
+  then obtain q where q_inadequate: "q \<in> gpda.states P\<^sub>0" "LR0_inadequate q" by blast
   from this(2) show False unfolding LR0_inadequate_def
   proof (standard, goal_cases shift_reduce reduce_reduce)
     case reduce_reduce
     then obtain X \<beta> Y \<delta> where conflict: "[X \<rightarrow> \<beta> \<cdot> []] \<in> q" "[Y \<rightarrow> \<delta> \<cdot> []] \<in> q" 
       "[X \<rightarrow> \<beta> \<cdot> []] \<noteq> [Y \<rightarrow> \<delta> \<cdot> []]" by fastforce
     then obtain \<gamma> where "reliable_prefix ([X \<rightarrow> \<beta> \<cdot> []]) \<gamma>"
-      "reliable_prefix ([Y \<rightarrow> \<delta> \<cdot> []]) \<gamma>" using state_imp_valids q_inadequate by auto
+      "reliable_prefix ([Y \<rightarrow> \<delta> \<cdot> []]) \<gamma>" using state_imp_valids q_inadequate 
+      by (auto simp: valids_def)
     then obtain \<gamma>' w \<nu> y where
       "Prods G' \<turnstile> [Nt S'] \<Rightarrow>r* \<gamma>' @ Nt X # map Tm w"
       "Prods G' \<turnstile> \<gamma>' @ Nt X # map Tm w \<Rightarrow>r \<gamma>' @ \<beta> @ map Tm w"
@@ -1808,43 +2120,6 @@ proof (rule ccontr)
       by (metis LR0 LR0_impossible(1,2) append_assoc same_append_eq)
   qed (use shift_reduce_imp_not_LR0 LR0 q_inadequate in auto)
 qed
-
-lemma derivers_appendD:
-  "(P \<turnstile> \<alpha> @ \<beta> \<Rightarrow>r* \<gamma>) = 
-    ((\<exists>\<beta>'. P \<turnstile> \<beta> \<Rightarrow>r* \<beta>' \<and> \<gamma> = \<alpha> @ \<beta>') \<or> (\<exists>\<alpha>' v. P \<turnstile> \<alpha> \<Rightarrow>r* \<alpha>' \<and> P \<turnstile> \<beta> \<Rightarrow>r* map Tm v \<and> \<gamma> = \<alpha>' @ map Tm v))" 
-  (is "_ = ?EX")
-proof
-  show "P \<turnstile> \<alpha> @ \<beta> \<Rightarrow>r* \<gamma> \<Longrightarrow> ?EX"
-  proof (induction "\<alpha> @ \<beta>" arbitrary: \<alpha> \<beta> rule: converse_rtranclp_induct)
-    case (step z)
-      show ?case proof (cases \<beta> rule: syms_rm_cases)
-        case (Tms w)
-        then show ?thesis using step(3)[of _ "map Tm w"] 
-          by (metis (no_types, lifting) derivern_append_map_Tm rtranclp.simps rtranclp_power 
-              rtranclp_trans step.hyps(1,2))
-      next
-        case (Nt \<beta>' A w)
-        with step obtain \<delta> where z_app: "P \<turnstile> \<beta> \<Rightarrow>r \<beta>' @ \<delta> @ map Tm w"  "z = \<alpha> @ \<beta>' @ \<delta> @ map Tm w"   
-          by (smt (verit, best) append.assoc deriver.cases deriver.intros rm_eq_imp_eq)
-        from step(3)[OF this(2)] consider 
-          \<beta>'' where "P \<turnstile> \<beta>' @ \<delta> @ map Tm w \<Rightarrow>r* \<beta>''" "\<gamma> = \<alpha> @ \<beta>''" |
-          \<alpha>'' v where "P \<turnstile> \<alpha>  \<Rightarrow>r* \<alpha>''" "P \<turnstile> \<beta>' @ \<delta> @ map Tm w \<Rightarrow>r* map Tm v"  "\<gamma> = \<alpha>'' @ map Tm v"  
-          using derivers_imp_derives derives_map_Tm_iff by blast
-        thus ?thesis using z_app by cases fastforce+
-      qed
-    qed simp
-next
-  assume ?EX
-  then show "P \<turnstile> \<alpha> @ \<beta> \<Rightarrow>r* \<gamma>" by standard 
-      (use derivers_prepend in blast, metis derivers_prepend derivers_append_map_Tm rtranclp_trans)
-qed
-
-lemma derivers_append_cases [consumes 1, case_names suffix prefix]:
-  assumes "P \<turnstile> \<alpha> @ \<beta> \<Rightarrow>r* \<gamma>"
-  obtains \<beta>' where "P \<turnstile> \<beta> \<Rightarrow>r* \<beta>'" "\<gamma> = \<alpha> @ \<beta>'" |
-    \<alpha>' v where "P \<turnstile> \<alpha> \<Rightarrow>r* \<alpha>'" "P \<turnstile> \<beta> \<Rightarrow>r* map Tm v" "\<gamma> = \<alpha>' @ map Tm v"
-  using derivers_appendD[THEN iffD1, OF assms] by blast
-
 
 lemma derivers_leftmost_derivers_last_step:
   assumes "Prods G' \<turnstile> Nt A # \<alpha> \<Rightarrow>r* \<beta>"
@@ -1878,15 +2153,15 @@ proof -
 qed
 
 lemma prefix_comp_unique_imp_eps:
-  assumes "LR0_adequate {i. reliable_prefix i \<alpha>}" (is "LR0_adequate ?p")
-    "reliable_prefix [X \<rightarrow> [] \<cdot> []] \<alpha>"
+  assumes "LR0_adequate (valids \<alpha>)" (is "LR0_adequate ?p")
+    "[X \<rightarrow> [] \<cdot> []] \<in> valids \<alpha>"
     "Prods G' \<turnstile> [Nt S'] \<Rightarrow>r* \<alpha> @ \<alpha>' @ Nt Y # map Tm x"
     "Prods G' \<turnstile> \<alpha> @ \<alpha>' @ Nt Y # map Tm x \<Rightarrow>r \<alpha> @ map Tm y"
   shows "\<alpha>' = [] \<and> Y = X \<and> x = y"
 proof -
   from assms(2) obtain w where X_derivers: "Prods G' \<turnstile> [Nt S'] \<Rightarrow>r* \<alpha> @ Nt X # map Tm w"
     "Prods G' \<turnstile> \<alpha> @ Nt X # map Tm w \<Rightarrow>r \<alpha> @ map Tm w" 
-    using reliable_prefixE by force
+    using reliable_prefixE unfolding valids_def by force
   from assms(3) show ?thesis proof (cases rule: stepcnt_cases)
     case refl
     with assms(4) have "\<alpha> @ map Tm y = [Nt S]" 
@@ -1903,23 +2178,25 @@ proof -
       by blast
     from assms(3,4) have deriver_y: "Prods G' \<turnstile> \<alpha>' @ Nt Y # map Tm x \<Rightarrow>r map Tm y"
       by (metis append_Nil deriver_prefix_indep)
-    have "?p \<in> npda.states P\<^sub>0" 
+    have "?p \<in> gpda.states P\<^sub>0" 
       using dfa_LR0.nextl_init_state nextl_dfa_LR0_is_valids by force
     with assms(1) show ?thesis proof (cases rule: LR0_adequate_cases)
       case (comp_unique B)
       with assms(2) have AX [simp]: "B = X"
         by auto
-      from A_reliable obtain Z'' where Z''_def [simp]: "Z' = Nt Z''" using comp_unique by auto
+      from A_reliable obtain Z'' where Z''_def [simp]: "Z' = Nt Z''" using comp_unique 
+         by (auto simp: valids_def)
       from A_reliable(3) deriver_y obtain \<gamma>' u v  where decomp: 
         "Prods G' \<turnstile> [Nt Z''] \<Rightarrow>r* \<gamma>'" "Prods G' \<turnstile> \<gamma>' \<Rightarrow>r map Tm u" 
         "Prods G' \<turnstile> \<gamma> @ map Tm z \<Rightarrow>r* map Tm v"
         "\<gamma>' @ map Tm v = \<alpha>' @ Nt Y # map Tm x" "y = u @ v"
         using derivers_leftmost_derivers_last_step[of Z'' "\<gamma> @ map Tm z" "\<alpha>' @ Nt Y # map Tm x" y] 
         unfolding Z''_def by metis
-      with comp_unique have "\<gamma>' = Nt X # map Tm u" using A_reliable by simp
+      with comp_unique have "\<gamma>' = Nt X # map Tm u" using A_reliable 
+        by (simp add: valids_def)
       with decomp show ?thesis 
         by (metis (no_types, lifting) append_Cons map_append rm_eq_imp_eq self_append_conv2)
-    qed (use assms(2) completes_def in fastforce, use A_reliable assms(2) in auto)
+    qed (use assms(2) completes_def in fastforce, use A_reliable assms(2) valids_def in auto)
   qed
 qed
 
@@ -1968,23 +2245,23 @@ proof (standard, goal_cases LR)
 qed
 
 lemma no_LR0_inadequate_states_imp_is_LR0:  
-  assumes adequates: "\<forall>q\<in>npda.states P\<^sub>0. LR0_adequate q"
+  assumes adequates: "\<forall>q\<in>gpda.states P\<^sub>0. LR0_adequate q"
   shows "is_LR 0" 
 proof (rule LRk_wlog, goal_cases LR)
   case (LR \<alpha> X \<beta> w \<gamma> Y x y \<delta>)
   obtain p where p_nextl: "dfa.nextl LR\<^sub>0 (dfa.init LR\<^sub>0) (\<alpha>@\<beta>) = p" by presburger
   with adequates have p_adequate: "LR0_adequate p" "p \<in> dfa.states LR\<^sub>0" using states_P0 
     using dfa_LR0.nextl_init_state by (metis Un_iff, metis)
-  hence p_P0: "p \<in> npda.states P\<^sub>0"
+  hence p_P0: "p \<in> gpda.states P\<^sub>0"
     by auto
-  from p_nextl have p_valids: "p = {i. reliable_prefix i (\<alpha>@\<beta>)}"
+  from p_nextl have p_valids: "p = valids (\<alpha>@\<beta>)"
     using nextl_dfa_LR0_is_valids by auto
   from LR have X_reliable: "reliable_prefix ([X \<rightarrow> \<beta> \<cdot> []]) (\<alpha>@\<beta>)" 
     using char_eq_reliable_prefix derivers_imp_char by auto
   from p_adequate(1) p_P0 show ?case proof cases
     case (singleton A \<alpha>')
     with X_reliable have singleton: "p = {[X \<rightarrow> \<beta> \<cdot> []]}" 
-      using p_nextl nextl_dfa_LR0_is_valids by force
+      using p_nextl nextl_dfa_LR0_is_valids unfolding valids_def by force
     from LR(6,8) obtain z where z_defs: "\<gamma> @ \<delta> = \<alpha> @ \<beta> @ map Tm z" "z @ x = y"
       using eq_hd_lt_imp_substring[of "\<alpha> @ \<beta>" "map Tm y" "\<gamma> @ \<delta>" "map Tm x"] append.assoc 
       by (metis (no_types, opaque_lifting) append_eq_map_conv map_Tm_inject_iff)
@@ -1992,24 +2269,24 @@ proof (rule LRk_wlog, goal_cases LR)
       case (1 u v)
       with derivers_substring_reliable[of "\<alpha> @ \<beta>" "map Tm u" Y x] LR(3)
       obtain B \<alpha>'' C \<beta>'' where "reliable_prefix [B \<rightarrow> \<alpha>'' \<cdot> C # \<beta>''] (\<alpha> @ \<beta>)" by fastforce
-      then show ?thesis using singleton p_valids by blast
+      then show ?thesis using singleton p_valids unfolding valids_def by blast
     next
       case (2 \<delta>')
       from LR(3) have "reliable_prefix [Y \<rightarrow> \<delta>' \<cdot> map Tm z] (\<alpha> @ \<beta>)" 
         using 2 LR(4,6) z_defs by fastforce
       with singleton p_valids have "z = [] \<and> \<delta>' = \<beta> \<and> X = Y" 
-        by (metis item.inject map_is_Nil_conv mem_Collect_eq singletonD)
+        by (metis item.inject map_is_Nil_conv mem_Collect_eq singletonD valids_def)
       with 2 z_defs show ?thesis by simp
     qed
   next
     case (comp_unique A)
     with p_valids X_reliable have comp_X: "completes p = {[X \<rightarrow> \<beta> \<cdot> []]}" "\<beta> = []"
-      unfolding completes_def by auto 
+      unfolding completes_def by (auto simp: valids_def) 
     from LR(6) have eq: "(\<alpha> @ \<beta>) @ map Tm y = \<gamma> @ \<delta> @ map Tm x" by simp
     show ?thesis proof (cases rule: substring_app_cases[OF eq LR(8)])
       case (1 _ _)
-      with prefix_comp_unique_imp_eps[OF p_adequate(1)[unfolded p_valids]] X_reliable
-        comp_X LR show ?thesis by (metis append.assoc append.right_neutral)
+      with prefix_comp_unique_imp_eps[OF p_adequate(1)[unfolded p_valids]] X_reliable comp_X LR 
+      show ?thesis by (metis append.assoc append.right_neutral completesD insertCI p_valids)
     next
       case (2 \<delta>\<^sub>1 x')
       from LR(3) have Y_reliable: "reliable_prefix [Y \<rightarrow> \<delta>\<^sub>1 \<cdot> map Tm x'] (\<alpha> @ \<beta>)" 
@@ -2020,29 +2297,29 @@ proof (rule LRk_wlog, goal_cases LR)
       show ?thesis proof (cases x')
         case Nil
         with Y_reliable p_valids have "[Y \<rightarrow> \<delta>\<^sub>1 \<cdot> map Tm x'] \<in> completes p" unfolding completes_def 
-          by simp
+          by (simp add: valids_def)
         with comp_X have "[Y \<rightarrow> \<delta>\<^sub>1 \<cdot> map Tm x'] = [X \<rightarrow> [] \<cdot> []]" by simp
         with 2 show ?thesis using comp_X by simp
       next
         case (Cons a x'')
         from Y_reliable p_valids have "[Y \<rightarrow> \<delta>\<^sub>1 \<cdot> Tm a # map Tm x''] \<in> noncompletes p"
-          unfolding Cons by auto
+          unfolding Cons by (auto simp: valids_def)
         then show ?thesis using comp_unique(2) sym.exhaust by blast
       qed
     qed
-  qed (use p_valids X_reliable completes_def in fastforce)
+  qed (use p_valids X_reliable completes_def valids_def in fastforce)
 qed
     
 
 theorem is_LR0_iff_no_LR0_inadequates:
-  "is_LR 0 = (\<forall>q\<in>npda.states P\<^sub>0. LR0_adequate q)"
+  "is_LR 0 = (\<forall>q\<in>gpda.states P\<^sub>0. LR0_adequate q)"
   using is_LR0_imp_no_LR0_inadequate_states no_LR0_inadequate_states_imp_is_LR0 by metis
 
 section \<open>Determinism of \<open>P\<^sub>0\<close> and Language Equivalence\<close>
 
 lemma LR_adequate_imp_P0_nxt_unique:
-  assumes "p \<in> npda.states P\<^sub>0" "LR0_adequate p"
-    "p # ps = ps' @ rs" "(ps', a, qs) \<in> npda.nxt P\<^sub>0" "(p # ps, a # w) \<turnstile>P c1"
+  assumes "p \<in> gpda.states P\<^sub>0" "LR0_adequate p"
+    "p # ps = ps' @ rs" "(ps', a, qs) \<in> gpda.nxt P\<^sub>0" "(p # ps, a # w) \<turnstile>P c1"
   shows "(qs @ rs, w) = c1"
   using assms(5) proof (cases, goal_cases qs'_nxt _)
   case (qs'_nxt ps'' qs' _)
@@ -2058,8 +2335,8 @@ next
 qed
 
 lemma LR_adequate_eps_tl_eq_imp_P0_eps_unique:
-  assumes "p \<in> npda.states P\<^sub>0" "LR0_adequate p"
-    "p # ps = p # ps0 @ rs0" "(p # ps0, qs0) \<in> npda.eps P\<^sub>0" "(p # ps0, qs1) \<in> npda.eps P\<^sub>0"
+  assumes "p \<in> gpda.states P\<^sub>0" "LR0_adequate p"
+    "p # ps = p # ps0 @ rs0" "(p # ps0, qs0) \<in> gpda.eps P\<^sub>0" "(p # ps0, qs1) \<in> gpda.eps P\<^sub>0"
   shows "qs0 @ rs0 = qs1 @ rs0"
   using assms(4) proof (cases rule: eps_P0E)
   case (reduce p'' ps'' X \<alpha>)
@@ -2093,15 +2370,15 @@ next
     with assms(2) qs_finish comp_singleton show ?thesis 
       by (metis (no_types, lifting) completes_singleton_imp_eq item.inject list.inject)
   next
-    case (finish _)
+    case finish
     then show ?thesis using qs_finish assms(4-) by fastforce
   qed
 qed
 
 lemma LR_adequate_imp_P0_eps_unique:
-  assumes "p \<in> npda.states P\<^sub>0" "LR0_adequate p"
-    and qs_eps: "p # ps = p # ps0 @ rs0" "(p # ps0, qs0) \<in> npda.eps P\<^sub>0"
-    and qs'_eps: "p # ps = p # ps1 @ rs1" "(p # ps1, qs1) \<in> npda.eps P\<^sub>0"
+  assumes "p \<in> gpda.states P\<^sub>0" "LR0_adequate p"
+    and qs_eps: "p # ps = p # ps0 @ rs0" "(p # ps0, qs0) \<in> gpda.eps P\<^sub>0"
+    and qs'_eps: "p # ps = p # ps1 @ rs1" "(p # ps1, qs1) \<in> gpda.eps P\<^sub>0"
   shows "qs0 @ rs0 = qs1 @ rs1"
 proof (cases "ps0 = ps1")
   case True
@@ -2137,7 +2414,7 @@ qed
 text \<open>If a state of \<open>P\<^sub>0\<close> is LR(0)-adequate, it behaves deterministically on that state:\<close>
 
 lemma LR0_adequate_imp_P0_step_unique:
-  assumes "p \<in> npda.states P\<^sub>0" "LR0_adequate p"
+  assumes "p \<in> gpda.states P\<^sub>0" "LR0_adequate p"
     "(p # ps, u) \<turnstile>P c0" "(p # ps, u) \<turnstile>P c1"
   shows "c0 = c1"
 using assms(3) proof (cases, goal_cases qs_nxt qs_eps)
@@ -2155,8 +2432,8 @@ using assms(3) proof (cases, goal_cases qs_nxt qs_eps)
 qed (use assms LR_adequate_imp_P0_nxt_unique in blast)
 
 theorem no_LR0_inadequates_imp_P0_stepn_unique:
-  assumes "\<forall>p \<in> npda.states P\<^sub>0. LR0_adequate p"
-    "set ps \<subseteq> npda.states P\<^sub>0"
+  assumes "\<forall>p \<in> gpda.states P\<^sub>0. LR0_adequate p"
+    "set ps \<subseteq> gpda.states P\<^sub>0"
     "(ps, u) \<turnstile>P(n) c0" "(ps, u) \<turnstile>P(n) c1"
   shows "c0 = c1"
   using assms(3-,2) proof (induction n arbitrary: ps u)
@@ -2169,11 +2446,11 @@ theorem no_LR0_inadequates_imp_P0_stepn_unique:
       "(ps, u) \<turnstile>P (p0 # ps0, u0)" "(p0 # ps0, u0) \<turnstile>P(n) c0"
       "(ps, u) \<turnstile>P (p1 # ps1, u1)" "(p1 # ps1, u1) \<turnstile>P(n) c1"
       using relpowp_Suc_D2 P0.step_imp_Cons by (smt (verit, ccfv_SIG) surj_pair)
-    moreover from Suc.prems(3) assms(1) have "p \<in> npda.states P\<^sub>0" "LR0_adequate p"
+    moreover from Suc.prems(3) assms(1) have "p \<in> gpda.states P\<^sub>0" "LR0_adequate p"
       by auto
     ultimately show thesis using that LR0_adequate_imp_P0_step_unique Cons by metis
   qed
-  moreover from this(1) Suc.prems(3) have "set ps' \<subseteq> npda.states P\<^sub>0"
+  moreover from this(1) Suc.prems(3) have "set ps' \<subseteq> gpda.states P\<^sub>0"
     using P0.step_states_imp_states by simp
   ultimately show ?case using Suc.IH by presburger
 qed simp
@@ -2181,44 +2458,350 @@ qed simp
 text \<open>If \<open>P\<^sub>0\<close> has no LR(0)-inadequate states, it is deterministic:\<close>
 
 corollary no_LR0_inadequates_imp_P0_deterministic:
-  assumes "\<forall>p \<in> npda.states P\<^sub>0. LR0_adequate p"
-    "([npda.init P\<^sub>0], w) \<turnstile>P(n) c0" "([npda.init P\<^sub>0], w) \<turnstile>P(n) c1"
+  assumes "\<forall>p \<in> gpda.states P\<^sub>0. LR0_adequate p"
+    "([gpda.init P\<^sub>0], w) \<turnstile>P(n) c0" "([gpda.init P\<^sub>0], w) \<turnstile>P(n) c1"
   shows "c0 = c1"
   using assms no_LR0_inadequates_imp_P0_stepn_unique[OF assms(1) _ assms(2-)] P0.init by simp
 
-thm shift_reduce.intros
+
 subsection \<open>Language Equivalence of \<open>P\<^sub>0\<close> and its Grammar\<close>
 
-lemma dfa_LR0_nxt_is_epsclo_of_shift:
-  assumes "Q \<in> dfa.states LR\<^sub>0"
-  shows "dfa.nxt LR\<^sub>0 Q Y = char_fa.epsclo {[X \<rightarrow> \<alpha> @ [Y] \<cdot> \<beta>]|X \<alpha> \<beta>. [X \<rightarrow> \<alpha> \<cdot> Y # \<beta>] \<in> Q}"
-proof -
-  from dfa_LR0_states_subset[OF assms(1)] char_fa.epsclo_idem
-  have "dfa.nxt LR\<^sub>0 Q Y = (\<Union>i \<in> Q. char_fa.epsclo (nfa.nxt char_fa i Y))"
-    unfolding dfa_LR0_nxt char_fa.nxt_Power_dfa char_fa.states_Power_dfa by blast
-  also have "... = char_fa.epsclo (\<Union>i \<in> Q. (nfa.nxt char_fa i Y))"
-    by auto
-  finally show ?thesis using char_fa_nxts_is_shifts 
-    by (metis (lifting) assms in_state_imp_in_It subsetI)
+lemma P0_step_cases [consumes 1, case_names shift reduce finish, cases set: P0.step]:
+  assumes "c\<^sub>0 \<turnstile>P c\<^sub>1"
+  obtains q qs a w where "c\<^sub>0 = (q # qs, a # w)" "c\<^sub>1 = (dfa.nxt LR\<^sub>0 q (Tm a) # q # qs, w)"
+    "q \<in> dfa.states LR\<^sub>0" "dfa.nxt LR\<^sub>0 q (Tm a) \<noteq> {}" |
+    p\<^sub>n ps p\<^sub>0 qs X \<alpha> w where "p\<^sub>0 = last (p\<^sub>n # ps)" "c\<^sub>0 = (p\<^sub>n # ps @ qs, w)" 
+    "c\<^sub>1 = (dfa.nxt LR\<^sub>0 p\<^sub>0 (Nt X) # p\<^sub>0 # qs, w)" "set (p\<^sub>n # ps) \<subseteq> dfa.states LR\<^sub>0"
+    "[X \<rightarrow> \<alpha> \<cdot> []] \<in> p\<^sub>n" "length \<alpha> = length ps" "X \<noteq> S'" |
+    q qs w where "c\<^sub>0 = (q # dfa.init LR\<^sub>0 # qs, w)" "c\<^sub>1 = ({[S' \<rightarrow> [] \<cdot> []]} # qs, w)"
+      "q \<in> dfa.states LR\<^sub>0" "[S' \<rightarrow> [Nt S] \<cdot> []] \<in> q"
+  using assms proof cases
+  case (step_nxt ps a qs rs w)
+  then show ?thesis using that(1) by fastforce
+next
+  case (step_eps ps qs rs w)
+  from this(3,1,2) show ?thesis using step_eps that(2-) 
+      by (cases rule: eps_P0E) auto
 qed
 
+lemma P0_final_step_is_finish:
+  assumes "(qs, u) \<turnstile>P ([{[S' \<rightarrow> [] \<cdot> []]}], [])" 
+  obtains q where "q \<in> dfa.states LR\<^sub>0" "(qs, u) = ([q, dfa.init LR\<^sub>0], [])" "[S' \<rightarrow> [Nt S] \<cdot> []] \<in> q"
+  using assms by cases auto
 
-lemma P0_imp_IPDA: (* Not true. Fix *)
-  assumes "(P # PS, u) \<turnstile>P* (Q # QS, v)"
-  obtains i j \<rho> \<sigma> where "i \<in> P" "j \<in> Q" "\<forall>n. \<rho> ! n \<in> PS ! n" "\<forall>n. \<sigma> ! n \<in> QS ! n"
-    "(i # \<rho>, u) \<turnstile>I* (j # \<sigma>, v)"
-  sorry
+lemma in_char_eps_imp_IPDA_reachable:
+  assumes "(i, j) \<in> (nfa.eps char_fa)\<^sup>*"
+  obtains \<sigma> where "(i # \<rho>, w) \<turnstile>I* (j # \<sigma> @ \<rho>, w)"
+  using assms proof (induction arbitrary: thesis rule: rtrancl_induct)
+  case base
+  from base[of "[]"] show ?case by simp
+next
+  case (step j k)
+  from step.hyps(2) obtain A \<alpha> X \<beta> \<gamma> where eps: "j = [A \<rightarrow> \<alpha> \<cdot> Nt X # \<beta>]" "k = [X \<rightarrow> [] \<cdot> \<gamma>]"
+    "(A, \<alpha> @ Nt X # \<beta>) \<in> Prods G'" "(X, \<gamma>) \<in> Prods G'" by blast
+  from step.IH obtain \<sigma> where "(i # \<rho>, w) \<turnstile>I* (j # \<sigma> @ \<rho>, w)" by blast
+  also from eps have "... \<turnstile>I (k # j # \<sigma> @ \<rho>, w)" 
+    using I.expanding by presburger
+  finally show ?case using step.prems[of "j # \<sigma>"] by simp
+qed
+
+(* TODO refactor *)
+lemma P0_stack_substr_reachable:
+  assumes "([gpda.init P\<^sub>0], u) \<turnstile>P(n) (p # ps @ q # qs, v)" "p \<in> dfa.states LR\<^sub>0"
+  obtains m u' where "m < n" "([gpda.init P\<^sub>0], u) \<turnstile>P(m) (q # qs, u')"
+    "(q # qs, u') \<turnstile>P(n - m) (p # ps @ q # qs, v)"
+  using assms proof (induction n arbitrary: p ps q qs v thesis)
+  case (Suc n)
+  note that = Suc.prems(1)
+  from Suc obtain c where n_steps: "([gpda.init P\<^sub>0], u) \<turnstile>P(n) c" "c \<turnstile>P (p # ps @ q # qs, v)"
+    by auto
+  from this(2) show ?case proof cases
+    case (shift r rs a w)
+    show ?thesis proof (cases ps)
+      case Nil
+      with shift have "r # rs = q # qs" by auto
+      note n_steps[unfolded shift this]
+      from Suc.prems(1)[OF _ this(1)] show thesis 
+        using shift n_steps(2) \<open>r # rs = q # qs\<close> by auto
+    next
+      case (Cons s ss)
+      with Suc.IH[of q qs s ss] obtain m u' where "m < n" "([gpda.init P\<^sub>0], u) \<turnstile>P(m) (q # qs, u')"
+        "(q # qs, u') \<turnstile>P(n - m) c" using n_steps shift by auto
+      then show ?thesis using n_steps(2) that 
+        using Suc_diff_le le_eq_less_or_eq less_Suc_eq by auto
+    qed
+  next
+    case (reduce r\<^sub>n rs r\<^sub>0 ss X \<alpha> w)
+    show ?thesis proof (cases ss)
+      case Nil
+      note ss_Nil = this
+      from reduce(3) have eqs [simp]: "p # ps = [dfa.nxt LR\<^sub>0 r\<^sub>0 (Nt X)]" "q # qs = [r\<^sub>0]" 
+        unfolding Nil by (simp_all add: append_eq_Cons_conv)
+      show ?thesis proof (cases rs rule: rev_cases)
+        case Nil
+        with reduce ss_Nil have "c = (q # qs, w)" by force
+        then show ?thesis using that[of n] n_steps by auto
+      next
+        case (snoc rs')
+        with ss_Nil reduce have "c = (r\<^sub>n # rs' @ q # qs, w)" by auto
+        with Suc.IH[OF _ n_steps(1)[unfolded this]] show ?thesis 
+          using that n_steps(2) Suc_diff_le le_eq_less_or_eq less_Suc_eq 
+            list.set_intros(1) reduce(4) relpowp_Suc_I subsetD by auto
+      qed
+    next
+      case (Cons a as)
+      note ss_Cons = this
+      show ?thesis proof (cases ps)
+        case Nil
+        with reduce(3) have rss[simp]: "r\<^sub>0 # ss = q # qs" by auto
+        show ?thesis proof (cases rs rule: rev_cases)
+          case Nil
+          with reduce rss have "c = (q # qs, w)" by force
+          then show ?thesis using n_steps that by fastforce
+        next
+          case (snoc rs' _)
+          with reduce rss have "c = (r\<^sub>n # rs' @ q # qs, w)" by fastforce
+          moreover from reduce have "r\<^sub>n \<in> dfa.states LR\<^sub>0" by fastforce
+          ultimately show ?thesis using that Suc.IH[of q qs r\<^sub>n rs' w] n_steps      
+            by (metis (no_types, lifting) Suc_diff_le less_Suc_eq_le less_or_eq_imp_le relpowp_Suc_I)
+        qed
+      next
+        case (Cons b bs)
+        with reduce(3) obtain ss' where q_substr: "ss = ss' @ q # qs" 
+          by auto
+        hence "c = (r\<^sub>n # (rs @ ss') @ q # qs, w)" using reduce by fastforce
+        moreover from reduce have "r\<^sub>n \<in> dfa.states LR\<^sub>0" by force
+        ultimately obtain m u' where 
+          "m < n" "([gpda.init P\<^sub>0], u) \<turnstile>P(m) (q # qs, u')" "(q # qs, u') \<turnstile>P(n - m) c"
+          using  Suc.IH[of q qs r\<^sub>n "rs @ ss'" w] n_steps reduce by blast
+        then show ?thesis using n_steps that Suc_diff_le le_eq_less_or_eq less_Suc_eq by auto
+      qed
+    qed
+  qed (use Suc(4) P0_final_item_notin_It in_state_imp_in_It in blast)
+qed simp
+
+lemma P0_stack_inc_Suc_0_or_dec:
+  assumes "(ps, u) \<turnstile>P (qs, v)" "length ps \<noteq> length qs"
+  shows "length ps > length qs \<or> length qs = Suc (length ps)"
+  using assms proof cases
+  case (reduce _ ps')
+  show ?thesis using assms(2) reduce by (cases ps') auto
+qed simp_all
+
+lemma tl_of_stack_contains_no_empty:
+  "\<lbrakk>([gpda.init P\<^sub>0], u) \<turnstile>P* (q # qs, v); q \<in> dfa.states LR\<^sub>0\<rbrakk> \<Longrightarrow> {} \<notin> set qs"
+proof (induction "q # qs" v arbitrary: q qs rule: rtranclp_induct2)
+  case (step ps v w)
+  from this(2) show ?case proof cases
+    case (shift r rs a x)
+    then show ?thesis using step by fastforce
+  next
+    case (reduce r\<^sub>n rs r\<^sub>0 ss X \<alpha> x)
+    then show ?thesis using step 
+      by (metis (no_types, lifting) ext Un_iff empty_iff last_in_set list.distinct(1) list.inject
+          list.set_intros(1) prod.inject set_ConsD set_append subset_eq)
+  next
+    case (finish r rs x)
+    then show ?thesis using step(4) step.hyps(3) by fastforce
+  qed
+qed simp
+
+
+  
+inductive stack_word :: "('n, 't) syms \<Rightarrow> ('n, 't) item set list \<times> 't list 
+  \<Rightarrow> ('n, 't) item set list \<times> 't list \<Rightarrow> bool" (\<open>_ \<Turnstile> _ \<turnstile>P* _\<close> 55)  where
+sw_refl [intro]: "[] \<Turnstile> c\<^sub>0 \<turnstile>P* c\<^sub>0" |
+sw_step: "\<lbrakk>\<alpha> \<Turnstile> c\<^sub>0 \<turnstile>P* (ps @ q # qs, u); (ps @ q # qs, u) \<turnstile>P (dfa.nxt LR\<^sub>0 q X # q # qs, v)\<rbrakk> 
+  \<Longrightarrow> X # drop (length ps) \<alpha> \<Turnstile> c\<^sub>0 \<turnstile>P* (dfa.nxt LR\<^sub>0 q X # q # qs, v)"
+
+inductive_cases stack_word_reflE [elim]: "[] \<Turnstile> c\<^sub>0 \<turnstile>P* c\<^sub>1"
+inductive_cases stack_word_stepE [elim]: "X # \<alpha> \<Turnstile> c\<^sub>0 \<turnstile>P* c\<^sub>1"
+
+lemma sw_stepI [intro]:
+  assumes "\<alpha> \<Turnstile> c\<^sub>0 \<turnstile>P* c\<^sub>1" "c\<^sub>1 \<turnstile>P c\<^sub>2"  
+    "c\<^sub>1 = (ps @ q # qs, u)" "c\<^sub>2 = (dfa.nxt LR\<^sub>0 q X # q # qs, v)" "\<alpha>' = drop (length ps) \<alpha>"
+  shows "X # \<alpha>' \<Turnstile> c\<^sub>0 \<turnstile>P* c\<^sub>2"
+  using assms sw_step by blast
+
+lemma stack_word_imp_P0_steps:
+  "\<alpha> \<Turnstile> c\<^sub>0 \<turnstile>P* c\<^sub>1 \<Longrightarrow> c\<^sub>0 \<turnstile>P* c\<^sub>1"
+  by (induction rule: stack_word.induct) auto
+
+lemma P0_steps_imp_stack_word:
+  assumes "c0 \<turnstile>P* (q # qs, w)" "q \<in> dfa.states LR\<^sub>0"
+  obtains \<alpha> where "\<alpha> \<Turnstile> c0 \<turnstile>P* (q # qs, w)"
+  using assms proof (induction "(q # qs, w)" arbitrary: thesis q qs w)
+  case (step c1)
+  note that = step.prems
+  note IH = step.hyps(3)
+  from step(2) show ?case proof cases
+    case (shift p ps a v)
+    with step obtain \<alpha> where sw: "\<alpha> \<Turnstile> c0 \<turnstile>P* ([] @ p # ps, a # w)" 
+      by auto
+    note step_unfolded = step[unfolded shift]
+    from sw have "Tm a # \<alpha> \<Turnstile> c0 \<turnstile>P* (q # qs, w)" unfolding shift
+      by standard (use step_unfolded shift(2) in auto)
+    then show ?thesis using that by simp
+  next
+    case (reduce p\<^sub>n ps p\<^sub>0 rs X \<alpha> v)
+    from reduce(1,2) obtain ps' where c1_snoc: "c1 = (ps' @ p\<^sub>0 # rs, v)" 
+      by (metis (no_types, lifting) append_Cons append_eq_append_conv2 list.distinct(1)
+          snoc_eq_iff_butlast)
+    with reduce step obtain \<alpha> where sw: "\<alpha> \<Turnstile> c0 \<turnstile>P* (ps' @ p\<^sub>0 # rs, v)" 
+      by (metis list.set_intros(1) subset_code(1))
+    note step_unfolded = step[unfolded reduce(3-) c1_snoc]
+    from sw have "Nt X # drop (length ps') \<alpha> \<Turnstile> c0 \<turnstile>P* (q # qs, w)" unfolding reduce(3)
+      by standard (use step_unfolded in simp_all)
+    then show ?thesis using that by simp
+  qed (use P0_final_item_notin_It in_state_imp_in_It that(2) in auto)
+qed fast
+      
+
+lemma P0_hd_is_valids_of_stack_word:
+  "\<alpha> \<Turnstile> ([gpda.init P\<^sub>0], u) \<turnstile>P* (q # qs, v) \<Longrightarrow> 
+    \<forall>n < length (q # qs). (q # qs) ! n  = valids (rev (drop n \<alpha>))"
+proof (induction "([gpda.init P\<^sub>0], u)" "(q # qs, v)" arbitrary: q qs u v rule: stack_word.induct)
+  case (sw_step \<alpha> ps q qs v X w)
+  from sw_step(3) show ?case proof cases
+    case (shift r rs a x)
+    with sw_step have ih: "\<forall>n < length (r # rs). (r # rs) ! n = valids (rev (drop n \<alpha>))" by blast
+    hence r_valids: "r = valids (rev \<alpha>)" by auto
+    from shift have drop_eq: "drop (length ps) \<alpha> = \<alpha>" by simp
+    from r_valids nxt_dfa_LR0_shift_is_valids_app shift(3) have 
+      "dfa.nxt LR\<^sub>0 q X = valids (rev (X # \<alpha>))"  
+      by (metis list.inject prod.inject rev.simps(2) shift(2))
+    hence "(dfa.nxt LR\<^sub>0 q X # q # qs) ! 0 = valids (rev (drop 0 (X # \<alpha>)))"
+      by simp
+    moreover from ih have "\<forall>n < length (q # qs). (q # qs) ! n = valids (rev (drop (Suc n) (X # \<alpha>)))"
+      using shift by auto
+    ultimately show ?thesis unfolding drop_eq        
+      by (smt (verit, ccfv_threshold) length_Suc_conv less_Suc_eq_0_disj nth_Cons_Suc)
+  next
+    case (reduce r\<^sub>n rs p\<^sub>0 ss Y \<beta> x)
+    from reduce(2) sw_step(2)[of r\<^sub>n "rs @ ss"] have ih_qqs:
+      "\<forall>n<length (q # qs). (q # qs) ! n = valids (rev (drop (length ps + n) \<alpha>))"
+        by (simp add: append_eq_conv_conj)
+    from reduce(1)[THEN last_of_Cons_idx_len_tl] have "p\<^sub>0 = (r\<^sub>n # rs @ ss) ! (length \<beta>)" 
+      using reduce(6) by (metis append_Cons length_Cons lessI nth_append_left)
+    with sw_step(2)[of r\<^sub>n "rs @ ss"] reduce(2,6) have p0_valids:
+      "p\<^sub>0 = valids (rev (drop (length ps) \<alpha>))"
+      by (metis add_Suc_right length_Cons length_append less_add_Suc1 list.inject nth_append_length
+          prod.inject reduce(3))
+    hence "dfa.nxt LR\<^sub>0 p\<^sub>0 X = valids (rev (X # drop (length ps) \<alpha>))"
+      using nxt_dfa_LR0_shift_is_valids_app reduce 
+      by (metis dfa_LR0.nextl_init_state nextl_dfa_LR0_is_valids rev.simps(2))
+    hence "(dfa.nxt LR\<^sub>0 q X # q # qs) ! 0 = valids (rev (drop 0 (X # drop (length ps) \<alpha>)))"
+      using reduce(3) by auto
+    moreover from ih_qqs have 
+      "\<forall>n<length (q # qs). (q # qs) ! n = valids (rev (drop (Suc n) (X # drop (length ps) \<alpha>)))" 
+      by (simp add: add.commute)
+    ultimately show ?thesis 
+      by (smt (verit, ccfv_threshold) length_Suc_conv less_Suc_eq_0_disj nth_Cons_Suc)
+  next
+    case (finish q qs w)
+    then show ?thesis using dfa_LR0_nxt_final_impossible_P0 
+      by (metis P0.steps_init_imp_states insert_subset list.inject list.simps(15) prod.inject
+          stack_word_imp_P0_steps sw_step.hyps(1))
+  qed
+qed (use init_P0_is_valids_empty valids_def in force)
+
+
+lemma P0_invariant:
+  "\<lbrakk>\<alpha> \<Turnstile> ([gpda.init P\<^sub>0], u @ v) \<turnstile>P* (q # qs, v); q \<noteq> {}\<rbrakk> \<Longrightarrow> Prods G' \<turnstile> rev \<alpha> \<Rightarrow>r* map Tm u"
+proof (induction "([gpda.init P\<^sub>0], u @ v)" "(q # qs, v)" arbitrary: q qs u v rule: stack_word.induct)
+  case (sw_step \<alpha> ps q qs w X v)
+  with stack_word_imp_P0_steps P0.reachable_imp_substring obtain u' where w_app: "u @ v = u' @ w"
+    by metis
+  with sw_step have \<alpha>_derivers: "Prods G' \<turnstile> rev \<alpha> \<Rightarrow>r* map Tm u'" 
+    by (smt (verit, ccfv_threshold) P0_step_cases empty_iff nxt_dfa_LR0_nempty_imp_ex_shift
+        prod.inject)
+  from sw_step(3) show ?case proof cases
+    case (shift r rs a x)
+    hence ps_Nil [simp]: "ps = []" and Xa [simp]: "X = Tm a" 
+      using inj_nxt_dfa_LR0_if_nempty by blast+ 
+    moreover from w_app shift have "u = u' @ [a]" by auto
+    ultimately show ?thesis
+      by (metis (no_types, lifting) \<alpha>_derivers derivers_append_map_Tm drop0 list.simps(8,9)
+          list.size(3) map_append rev.simps(2)) 
+  next
+    case (reduce p\<^sub>n rs p\<^sub>0 ss Y \<beta> x)
+    moreover from this obtain \<alpha>' where "\<alpha> = rev \<beta> @ \<alpha>'"
+    proof -
+      have "p\<^sub>n = (p\<^sub>n # rs @ ss) ! 0" by simp
+      with P0_hd_is_valids_of_stack_word[of _ _ p\<^sub>n "rs @ ss"] reduce sw_step have 
+        "reliable_prefix [Y \<rightarrow> \<beta> \<cdot> []] (rev \<alpha>)"
+        by (metis drop0 length_greater_0_conv list.distinct(1) validD)
+      then obtain \<alpha>' where "rev \<alpha> = \<alpha>' @ \<beta>"  
+        by (blast elim: reliable_prefixE)
+      thus thesis using that rev_eq_append_conv by blast
+    qed
+    moreover have "length ps = length rs" 
+      by (cases rs rule: rev_cases) (use reduce in auto)
+    ultimately have \<alpha>_app: "\<alpha> = rev \<beta> @ drop (length ps) \<alpha>" 
+      by simp
+    from reduce have Y_deriver: "Prods G' \<turnstile> [Nt Y] \<Rightarrow>r \<beta>" 
+      using in_state_imp_in_It in_It_imp_in_Prods deriver_singleton by fastforce
+    from reduce have XY: "X = Nt Y" using
+        inj_nxt_dfa_LR0_if_nempty[OF _ _ sw_step(4), of "Nt Y"] last_in_set by blast
+    with \<alpha>_app have "rev (X # drop (length ps) \<alpha>) = rev (drop (length ps) \<alpha>) @ [Nt Y]" 
+      by simp
+    also from Y_deriver have "Prods G' \<turnstile> rev (drop (length ps) \<alpha>) @ [Nt Y] 
+      \<Rightarrow>r rev (drop (length ps) \<alpha>) @ \<beta>" by (simp add: deriver_singleton deriver_snoc_Nt)
+    also have "... = rev \<alpha>" using \<alpha>_app 
+      by (metis rev_append rev_rev_ident)
+    also note \<alpha>_derivers
+    finally show ?thesis using w_app reduce by fast
+  next
+    case (finish r rs x)
+    moreover from sw_step(1) P0.steps_init_imp_states have "q \<in> gpda.states P\<^sub>0" 
+      using stack_word_imp_P0_steps by (meson in_mono in_set_conv_decomp)
+    ultimately show ?thesis using dfa_LR0_nxt_final_impossible_P0 by blast
+  qed
+qed simp
+
+lemma P0_init_stack_word_length_inv:
+  "\<alpha> \<Turnstile> ([gpda.init P\<^sub>0], u) \<turnstile>P* (qs, v) \<Longrightarrow> Suc (length \<alpha>) = length qs"
+  by (induction "([gpda.init P\<^sub>0], u)" "(qs, v)" arbitrary: qs v rule: stack_word.induct) auto
+
+
+lemma P0_init_reaches_S'S_comp_imp_derivers:
+  assumes "([gpda.init P\<^sub>0], w) \<turnstile>P* ([q, dfa.init LR\<^sub>0], [])"
+    "q \<in> dfa.states LR\<^sub>0" "[S' \<rightarrow> [Nt S] \<cdot> []] \<in> q"
+  shows "Prods G' \<turnstile> [Nt S] \<Rightarrow>r* map Tm w"
+using assms(1,2) proof (cases rule: P0_steps_imp_stack_word)
+  case (1 \<alpha>)
+  from P0_init_stack_word_length_inv[OF 1] obtain X where "\<alpha> = [X]" 
+  proof -
+    note P0_init_stack_word_length_inv[OF 1]
+    hence "length \<alpha> = Suc 0" by simp
+    then show thesis using that 
+      by (metis Suc_length_conv length_0_conv)
+  qed
+  note stack_word = 1[unfolded this]
+  then show ?thesis proof cases
+    case (sw_step \<alpha> ps u)
+    hence "X = Nt S" 
+      by (metis S'_complete_reliable_imp_S assms(3) dfa_LR0.init dfa_LR0_init_reliable_Nil list.inject
+          nxt_dfa_LR0_shift_is_valids_app self_append_conv2 state_imp_valids validD)
+    with P0_invariant[of "[Nt S]" w "[]"] show ?thesis using stack_word assms(3) by auto
+  qed
+qed
+
 
 lemma P0_Lang_subset_Lang_G:
   "P0.Lang \<subseteq> LangS G'"
 proof
   fix w
   assume "w \<in> P0.Lang"
-  hence "([npda.init P\<^sub>0], w) \<turnstile>P* ([{[S' \<rightarrow> [] \<cdot> []]}], [])"
+  hence "([gpda.init P\<^sub>0], w) \<turnstile>P* ([{[S' \<rightarrow> [] \<cdot> []]}], [])"
     unfolding P0.Lang_def by auto
-  show "w \<in> LangS G'" sorry
+  then obtain q where "([gpda.init P\<^sub>0], w) \<turnstile>P* ([q, dfa.init LR\<^sub>0], [])"
+    "q \<in> dfa.states LR\<^sub>0" "[S' \<rightarrow> [Nt S] \<cdot> []] \<in> q"
+    by cases (use P0_init_not_final in force, use P0_final_step_is_finish in force)
+  then show "w \<in> LangS G'" 
+    using P0_init_reaches_S'S_comp_imp_derivers 
+      G'_derives_from_S_imp_in_Lang derivers_imp_derives by blast
 qed
-
 
 theorem P0_Lang_eq_Lang_G:
   "P0.Lang = LangS G'"
@@ -2228,9 +2811,6 @@ proof
   show "LangS G' \<subseteq> P0.Lang"
     sorry
 qed
-
-
-
 
 end
 end
